feat: rsi_rtt_set_ripas_spec

container/coq/pointer/Layer9/Spec.v
@@ -1,3 +1,4 @@
+Require Import Bottom.Spec.
 Require Import CommonDeps.
 Require Import DataTypes.
 Require Import GlobalDefs.
@@ -12,368 +13,355 @@ Require Import Layer8.Spec.
 Local Open Scope string_scope.
 Local Open Scope Z_scope.
 
+Parameter check_rcsm_mask_para : abs_PA_t -> bool.
+
 Section Layer9_Spec.
 
   Context `{int_ptr: IntPtrCast}.
 
-  Definition rsi_rtt_create_spec (v_0_Zptr: Z) (v_1_Zptr: Z) (v_2: Z) (v_3: Z) (st: RData) : (option (Z * RData)) :=
-    when v__0, st_0 == (
-        if (((test_PA v_1_Zptr) & (1)) =? (0))
+  Definition map_unmap_ns_s1_0_low (st_0: RData) (st_12: RData) (v_17: Ptr) (v_3: abs_PTE_t) (v_31: Z) (v__sroa_0_0_copyload: Ptr) (v__sroa_7_0_copyload: Z) : (option (Z * RData)) :=
+    rely (((v_31 =? (0)) = (true)));
+    when st_14 == ((stage1_tlbi_all_spec st_12));
+    when st_15 == ((__tte_write_spec_abs (ptr_offset v_17 (8 * (v__sroa_7_0_copyload))) v_3 st_14));
+    when st_16 == ((iasm_8_spec st_15));
+    when st_17 == ((iasm_12_isb_spec st_16));
+    when st_18 == ((__granule_get_spec v__sroa_0_0_copyload st_17));
+    when st_19 == ((granule_unlock_spec v__sroa_0_0_copyload st_18));
+    when st_20 == ((free_stack "map_unmap_ns_s1" st_0 st_19));
+    (Some (0, st_20)).
+
+  Definition map_unmap_ns_s1_1_low (st_0: RData) (st_11: RData) (v_17: Ptr) (v_3: abs_PTE_t) (v__sroa_0_0_copyload: Ptr) (v__sroa_7_0_copyload: Z) : (option (Z * RData)) :=
+    when st_13 == ((stage1_tlbi_all_spec st_11));
+    when st_14 == ((__tte_write_spec_abs (ptr_offset v_17 (8 * (v__sroa_7_0_copyload))) v_3 st_13));
+    when st_15 == ((iasm_8_spec st_14));
+    when st_16 == ((iasm_12_isb_spec st_15));
+    when st_17 == ((__granule_get_spec v__sroa_0_0_copyload st_16));
+    when st_18 == ((granule_unlock_spec v__sroa_0_0_copyload st_17));
+    when st_19 == ((free_stack "map_unmap_ns_s1" st_0 st_18));
+    (Some (0, st_19)).
+
+  Definition map_unmap_ns_s1_2_low (st_0: RData) (st_12: RData) (v_17: Ptr) (v_47: Z) (v__sroa_0_0_copyload: Ptr) (v__sroa_7_0_copyload: Z) : (option (Z * RData)) :=
+    rely (((v_47 =? (0)) = (true)));
+    when v_51, st_14 == ((s2tte_create_unassigned_spec_abs 1 st_12));
+    when st_15 == ((__tte_write_spec_abs (ptr_offset v_17 (8 * (v__sroa_7_0_copyload))) v_51 st_14));
+    when st_16 == ((iasm_8_spec st_15));
+    when st_17 == ((iasm_12_isb_spec st_16));
+    when st_18 == ((stage1_tlbi_all_spec st_17));
+    when st_19 == ((__granule_put_spec v__sroa_0_0_copyload st_18));
+    when st_20 == ((granule_unlock_spec v__sroa_0_0_copyload st_19));
+    when st_21 == ((free_stack "map_unmap_ns_s1" st_0 st_20));
+    (Some (0, st_21)).
+
+  Definition map_unmap_ns_s1_3_low (st_0: RData) (st_11: RData) (v_17: Ptr) (v_20: abs_PTE_t) (v__sroa_0_0_copyload: Ptr) (v__sroa_7_0_copyload: Z) : (option (Z * RData)) :=
+    when v_51, st_13 == ((s2tte_create_unassigned_spec_abs 1 st_11));
+    when st_14 == ((__tte_write_spec_abs (ptr_offset v_17 (8 * (v__sroa_7_0_copyload))) v_51 st_13));
+    when st_15 == ((iasm_8_spec st_14));
+    when st_16 == ((iasm_12_isb_spec st_15));
+    when st_17 == ((stage1_tlbi_all_spec st_16));
+    when st_18 == ((__granule_put_spec v__sroa_0_0_copyload st_17));
+    when st_19 == ((granule_unlock_spec v__sroa_0_0_copyload st_18));
+    when st_20 == ((free_stack "map_unmap_ns_s1" st_0 st_19));
+    (Some (0, st_20)).
+
+  Definition rsi_rtt_set_ripas_0 (st_0: RData) (st_10: RData) (v_34: Ptr) (v_38: bool) (v__sroa_0_0_copyload: Ptr) (v__sroa_3_0_copyload: Z) (tte_to_write: abs_PTE_t) : (option (Z * RData)) :=
+    rely ((v_38 = (true)));
+    when st_16 == (
+        (granule_unlock_spec
+          v__sroa_0_0_copyload
+          (st_10.[share].[granule_data] :<
+            (((st_10.(share)).(granule_data)) #
+              (((v_34.(poffset)) + ((8 * (v__sroa_3_0_copyload)))) / (4096)) ==
+              ((((st_10.(share)).(granule_data)) @ (((v_34.(poffset)) + ((8 * (v__sroa_3_0_copyload)))) / (4096))).[g_norm] :<
+                (((((st_10.(share)).(granule_data)) @ (((v_34.(poffset)) + ((8 * (v__sroa_3_0_copyload)))) / (4096))).(g_norm)) #
+                  (((v_34.(poffset)) + ((8 * (v__sroa_3_0_copyload)))) mod (4096)) ==
+                  (test_PTE_Z tte_to_write)))))));
+    (Some (0, st_16)).
+
+  Definition rsi_rtt_set_ripas_1 (st_0: RData) (st_14: RData) (v_34: Ptr) (v_38: bool) (v__sroa_0_0_copyload: Ptr) (v__sroa_3_0_copyload: Z) (tte_to_write: abs_PTE_t) : (option (Z * RData)) :=
+    rely ((v_38 = (true)));
+    when st_19 == (
+        (granule_unlock_spec
+          v__sroa_0_0_copyload
+          (st_14.[share].[granule_data] :<
+            (((st_14.(share)).(granule_data)) #
+              (((v_34.(poffset)) + ((8 * (v__sroa_3_0_copyload)))) / (4096)) ==
+              ((((st_14.(share)).(granule_data)) @ (((v_34.(poffset)) + ((8 * (v__sroa_3_0_copyload)))) / (4096))).[g_norm] :<
+                (((((st_14.(share)).(granule_data)) @ (((v_34.(poffset)) + ((8 * (v__sroa_3_0_copyload)))) / (4096))).(g_norm)) #
+                  (((v_34.(poffset)) + ((8 * (v__sroa_3_0_copyload)))) mod (4096)) ==
+                  (test_PTE_Z tte_to_write)))))));
+    (Some (0, st_19)).
+
+  Definition rsi_rtt_set_ripas_spec (v_0: Z) (v_1: Z) (v_2: Z) (v_3: Z) (st: RData) : (option (Z * RData)) :=
+    if (v_3 >? (1))
+    then (Some (1, st))
+    else (
+      if (check_rcsm_mask_para (test_PA v_0))
+      then (
+        when st_1 == ((spinlock_acquire_spec (mkPtr "granules" ((test_PA v_0).(meta_granule_offset))) st));
+        if (((((((st_1.(share)).(globals)).(g_granules)) @ (((test_PA v_0).(meta_granule_offset)) / (16))).(e_state_s_granule)) - (5)) =? (0))
         then (
-          when v_18, st_0 == (
-              when ret, st' == ((granule_try_lock_spec (mkPtr "granules" ((test_PA v_1_Zptr).(meta_granule_offset))) 5 st));
-              if ret
-              then (Some ((mkPtr "granules" ((test_PA v_1_Zptr).(meta_granule_offset))), st'))
-              else (Some ((mkPtr "null" 0), st')));
-          rely (((((v_18.(poffset)) mod (16)) = (0)) /\ (((v_18.(poffset)) >= (0)))));
-          rely ((((v_18.(pbase)) = ("granules")) \/ (((v_18.(pbase)) = ("null")))));
-          when v__1, st_1 == (
-              if (((v_18.(pbase)) =? ("null")) /\ (((v_18.(poffset)) =? (0))))
-              then (Some ((pack_struct_return_code_para (make_return_code_para 1)), st_0))
+          rely ((((((test_PA v_0).(meta_granule_offset)) mod (16)) = (0)) /\ ((((test_PA v_0).(meta_granule_offset)) >= (0)))));
+          when rtt_ret, st_3 == ((rtt_walk_lock_unlock_spec_abs (mkPtr "stack_s_rtt_walk" 0) (mkPtr "granules" ((test_PA v_0).(meta_granule_offset))) 0 64 v_1 v_2 st_1));
+          if (((rtt_ret.(e_1)) - (v_2)) =? (0))
+          then (
+            if ((v_2 <? (3)) && ((((abs_tte_read (mkPtr "granule_data" (((rtt_ret.(e_2)).(poffset)) + ((8 * ((rtt_ret.(e_3))))))) st_3).(meta_desc_type)) =? (3))))
+            then (
+              when st_13 == ((granule_unlock_spec (rtt_ret.(e_2)) st_3));
+              (Some ((pack_struct_return_code_para (make_return_code_para 8)), st_13)))
+            else (
+              if ((v_2 =? (3)) && ((((abs_tte_read (mkPtr "granule_data" (((rtt_ret.(e_2)).(poffset)) + ((8 * ((rtt_ret.(e_3))))))) st_3).(meta_desc_type)) =? (3))))
+              then (
+                if (v_3 =? (0))
+                then (
+                  when st_16 == (
+                      (granule_unlock_spec
+                        (rtt_ret.(e_2))
+                        (st_3.[share].[granule_data] :<
+                          (((st_3.(share)).(granule_data)) #
+                            ((((rtt_ret.(e_2)).(poffset)) + ((8 * ((rtt_ret.(e_3)))))) / (4096)) ==
+                            ((((st_3.(share)).(granule_data)) @ ((((rtt_ret.(e_2)).(poffset)) + ((8 * ((rtt_ret.(e_3)))))) / (4096))).[g_norm] :<
+                              (((((st_3.(share)).(granule_data)) @ ((((rtt_ret.(e_2)).(poffset)) + ((8 * ((rtt_ret.(e_3)))))) / (4096))).(g_norm)) #
+                                ((((rtt_ret.(e_2)).(poffset)) + ((8 * ((rtt_ret.(e_3)))))) mod (4096)) ==
+                                (test_PTE_Z (mkabs_PTE_t ((abs_tte_read (mkPtr "granule_data" (((rtt_ret.(e_2)).(poffset)) + ((8 * ((rtt_ret.(e_3))))))) st_3).(meta_PA)) 0 0 1))))))));
+                  (Some (0, st_16)))
+                else (
+                  when st_16 == (
+                      (granule_unlock_spec
+                        (rtt_ret.(e_2))
+                        (st_3.[share].[granule_data] :<
+                          (((st_3.(share)).(granule_data)) #
+                            ((((rtt_ret.(e_2)).(poffset)) + ((8 * ((rtt_ret.(e_3)))))) / (4096)) ==
+                            ((((st_3.(share)).(granule_data)) @ ((((rtt_ret.(e_2)).(poffset)) + ((8 * ((rtt_ret.(e_3)))))) / (4096))).[g_norm] :<
+                              (((((st_3.(share)).(granule_data)) @ ((((rtt_ret.(e_2)).(poffset)) + ((8 * ((rtt_ret.(e_3)))))) / (4096))).(g_norm)) #
+                                ((((rtt_ret.(e_2)).(poffset)) + ((8 * ((rtt_ret.(e_3)))))) mod (4096)) ==
+                                (test_PTE_Z (abs_tte_read (mkPtr "granule_data" (((rtt_ret.(e_2)).(poffset)) + ((8 * ((rtt_ret.(e_3))))))) st_3))))))));
+                  (Some (0, st_16))))
               else (
-                when v_23, st_1 == (
-                    when ret, st' == ((granule_try_lock_spec (mkPtr "granules" ((test_PA v_0_Zptr).(meta_granule_offset))) 1 st_0));
-                    if ret
+                if ((v_2 <>? (3)) && ((((abs_tte_read (mkPtr "granule_data" (((rtt_ret.(e_2)).(poffset)) + ((8 * ((rtt_ret.(e_3))))))) st_3).(meta_desc_type)) =? (1))))
+                then (
+                  if (v_3 =? (0))
+                  then (
+                    rely ((true = (true)));
+                    when st_16 == (
+                        (granule_unlock_spec
+                          (rtt_ret.(e_2))
+                          (st_3.[share].[granule_data] :<
+                            (((st_3.(share)).(granule_data)) #
+                              ((((rtt_ret.(e_2)).(poffset)) + ((8 * ((rtt_ret.(e_3)))))) / (4096)) ==
+                              ((((st_3.(share)).(granule_data)) @ ((((rtt_ret.(e_2)).(poffset)) + ((8 * ((rtt_ret.(e_3)))))) / (4096))).[g_norm] :<
+                                (((((st_3.(share)).(granule_data)) @ ((((rtt_ret.(e_2)).(poffset)) + ((8 * ((rtt_ret.(e_3)))))) / (4096))).(g_norm)) #
+                                  ((((rtt_ret.(e_2)).(poffset)) + ((8 * ((rtt_ret.(e_3)))))) mod (4096)) ==
+                                  (test_PTE_Z (mkabs_PTE_t ((abs_tte_read (mkPtr "granule_data" (((rtt_ret.(e_2)).(poffset)) + ((8 * ((rtt_ret.(e_3))))))) st_3).(meta_PA)) 0 0 1))))))));
+                    (Some (0, st_16)))
+                  else (
+                    rely ((true = (true)));
+                    when st_16 == (
+                        (granule_unlock_spec
+                          (rtt_ret.(e_2))
+                          (st_3.[share].[granule_data] :<
+                            (((st_3.(share)).(granule_data)) #
+                              ((((rtt_ret.(e_2)).(poffset)) + ((8 * ((rtt_ret.(e_3)))))) / (4096)) ==
+                              ((((st_3.(share)).(granule_data)) @ ((((rtt_ret.(e_2)).(poffset)) + ((8 * ((rtt_ret.(e_3)))))) / (4096))).[g_norm] :<
+                                (((((st_3.(share)).(granule_data)) @ ((((rtt_ret.(e_2)).(poffset)) + ((8 * ((rtt_ret.(e_3)))))) / (4096))).(g_norm)) #
+                                  ((((rtt_ret.(e_2)).(poffset)) + ((8 * ((rtt_ret.(e_3)))))) mod (4096)) ==
+                                  (test_PTE_Z (abs_tte_read (mkPtr "granule_data" (((rtt_ret.(e_2)).(poffset)) + ((8 * ((rtt_ret.(e_3))))))) st_3))))))));
+                    (Some (0, st_16))))
+                else (
+                  if (
+                    (((((abs_tte_read (mkPtr "granule_data" (((rtt_ret.(e_2)).(poffset)) + ((8 * ((rtt_ret.(e_3))))))) st_3).(meta_desc_type)) =? (0)) &&
+                      ((((abs_tte_read (mkPtr "granule_data" (((rtt_ret.(e_2)).(poffset)) + ((8 * ((rtt_ret.(e_3))))))) st_3).(meta_ripas)) =? (0)))) &&
+                      ((((abs_tte_read (mkPtr "granule_data" (((rtt_ret.(e_2)).(poffset)) + ((8 * ((rtt_ret.(e_3))))))) st_3).(meta_mem_attr)) =? (0)))))
+                  then (
+                    when st_16 == (
+                        (granule_unlock_spec
+                          (rtt_ret.(e_2))
+                          (st_3.[share].[granule_data] :<
+                            (((st_3.(share)).(granule_data)) #
+                              ((((rtt_ret.(e_2)).(poffset)) + ((8 * ((rtt_ret.(e_3)))))) / (4096)) ==
+                              ((((st_3.(share)).(granule_data)) @ ((((rtt_ret.(e_2)).(poffset)) + ((8 * ((rtt_ret.(e_3)))))) / (4096))).[g_norm] :<
+                                (((((st_3.(share)).(granule_data)) @ ((((rtt_ret.(e_2)).(poffset)) + ((8 * ((rtt_ret.(e_3)))))) / (4096))).(g_norm)) #
+                                  ((((rtt_ret.(e_2)).(poffset)) + ((8 * ((rtt_ret.(e_3)))))) mod (4096)) ==
+                                  (test_PTE_Z
+                                    (mkabs_PTE_t
+                                      ((abs_tte_read (mkPtr "granule_data" (((rtt_ret.(e_2)).(poffset)) + ((8 * ((rtt_ret.(e_3))))))) st_3).(meta_PA))
+                                      ((abs_tte_read (mkPtr "granule_data" (((rtt_ret.(e_2)).(poffset)) + ((8 * ((rtt_ret.(e_3))))))) st_3).(meta_desc_type))
+                                      v_3
+                                      ((abs_tte_read (mkPtr "granule_data" (((rtt_ret.(e_2)).(poffset)) + ((8 * ((rtt_ret.(e_3))))))) st_3).(meta_mem_attr))))))))));
+                    (Some (0, st_16)))
+                  else (
+                    if (
+                      (((((abs_tte_read (mkPtr "granule_data" (((rtt_ret.(e_2)).(poffset)) + ((8 * ((rtt_ret.(e_3))))))) st_3).(meta_desc_type)) =? (0)) &&
+                        ((((abs_tte_read (mkPtr "granule_data" (((rtt_ret.(e_2)).(poffset)) + ((8 * ((rtt_ret.(e_3))))))) st_3).(meta_ripas)) =? (0)))) &&
+                        ((((abs_tte_read (mkPtr "granule_data" (((rtt_ret.(e_2)).(poffset)) + ((8 * ((rtt_ret.(e_3))))))) st_3).(meta_mem_attr)) =? (1)))))
                     then (
-                      when ret_record, st_4 == ((rtt_walk_lock_unlock_spec_abs (mkPtr "stack_s_rtt_walk" 0) v_18 0 64 v_2 v_3 st'));
-                      rely ((((ret_record.(e_2)).(pbase)) =s ("granules")));
-                      rely (((((ret_record.(e_2)).(poffset)) mod (16)) = (0)));
-                      rely ((((ret_record.(e_1)) <= (3)) /\ (((ret_record.(e_1)) >= (0)))));
-                      if (((ret_record.(e_1)) - ((v_3 + ((- 1))))) =? (0))
-                      then (
-                        if (
-                          ((((abs_tte_read (mkPtr "granule_data" (((ret_record.(e_2)).(poffset)) + ((8 * ((ret_record.(e_3))))))) st_4).(meta_desc_type)) =? (0)) &&
-                            ((((abs_tte_read (mkPtr "granule_data" (((ret_record.(e_2)).(poffset)) + ((8 * ((ret_record.(e_3))))))) st_4).(meta_ripas)) =? (0)))))
-                        then (
-                          when st_10 == (
-                              (s2tt_init_unassigned_spec
-                                (mkPtr "granule_data" ((test_PA v_0_Zptr).(meta_granule_offset)))
-                                ((abs_tte_read (mkPtr "granule_data" (((ret_record.(e_2)).(poffset)) + ((8 * ((ret_record.(e_3))))))) st_4).(meta_ripas))
-                                st_4));
-                          rely ((((((ret_record.(e_2)).(poffset)) + (8)) mod (16)) = (8)));
-                          rely (((((test_PA v_0_Zptr).(meta_granule_offset)) mod (16)) = (0)));
-                          when st_16 == (
-                              (granule_unlock_spec
-                                (ret_record.(e_2))
-                                ((st_10.[share].[globals].[g_granules] :<
-                                  (((((st_10.(share)).(globals)).(g_granules)) #
-                                    ((((ret_record.(e_2)).(poffset)) + (8)) / (16)) ==
-                                    (((((st_10.(share)).(globals)).(g_granules)) @ ((((ret_record.(e_2)).(poffset)) + (8)) / (16))).[e_ref] :<
-                                      ((((((st_10.(share)).(globals)).(g_granules)) @ ((((ret_record.(e_2)).(poffset)) + (8)) / (16))).(e_ref)).[e_u_anon_3_0] :<
-                                        (((((((st_10.(share)).(globals)).(g_granules)) @ ((((ret_record.(e_2)).(poffset)) + (8)) / (16))).(e_ref)).(e_u_anon_3_0)) + (1))))) #
-                                    ((((test_PA v_0_Zptr).(meta_granule_offset)) + (4)) / (16)) ==
-                                    ((((((st_10.(share)).(globals)).(g_granules)) #
-                                      ((((ret_record.(e_2)).(poffset)) + (8)) / (16)) ==
-                                      (((((st_10.(share)).(globals)).(g_granules)) @ ((((ret_record.(e_2)).(poffset)) + (8)) / (16))).[e_ref] :<
-                                        ((((((st_10.(share)).(globals)).(g_granules)) @ ((((ret_record.(e_2)).(poffset)) + (8)) / (16))).(e_ref)).[e_u_anon_3_0] :<
-                                          (((((((st_10.(share)).(globals)).(g_granules)) @ ((((ret_record.(e_2)).(poffset)) + (8)) / (16))).(e_ref)).(e_u_anon_3_0)) + (1))))) @ ((((test_PA v_0_Zptr).(meta_granule_offset)) + (4)) / (16))).[e_state_s_granule] :<
-                                      5))).[share].[granule_data] :<
-                                  (((st_10.(share)).(granule_data)) #
-                                    ((((ret_record.(e_2)).(poffset)) + ((8 * ((ret_record.(e_3)))))) / (4096)) ==
-                                    ((((st_10.(share)).(granule_data)) @ ((((ret_record.(e_2)).(poffset)) + ((8 * ((ret_record.(e_3)))))) / (4096))).[g_norm] :<
-                                      (((((st_10.(share)).(granule_data)) @ ((((ret_record.(e_2)).(poffset)) + ((8 * ((ret_record.(e_3)))))) / (4096))).(g_norm)) #
-                                        ((((ret_record.(e_2)).(poffset)) + ((8 * ((ret_record.(e_3)))))) mod (4096)) ==
-                                        (test_PTE_Z (mkabs_PTE_t (test_PA v_0_Zptr) 3 0))))))));
-                          when st_17 == ((granule_unlock_spec (mkPtr "granules" ((test_PA v_0_Zptr).(meta_granule_offset))) st_16));
-                          (Some (0, st_17)))
-                        else (
-                          if (((v_3 + ((- 1))) <? (3)) && ((((abs_tte_read (mkPtr "granule_data" (((ret_record.(e_2)).(poffset)) + ((8 * ((ret_record.(e_3))))))) st_4).(meta_desc_type)) =? (3))))
-                          then (
-                            match (
-                              match (
-                                when st_11 == ((granule_unlock_spec (ret_record.(e_2)) st_4));
-                                when st_12 == ((granule_unlock_spec (mkPtr "granules" ((test_PA v_0_Zptr).(meta_granule_offset))) st_11));
-                                (Some (true, (pack_struct_return_code_para (make_return_code_para 9)), st_12))
-                              ) with
-                              | (Some (return___1, retval___1, st_10)) => (Some (return___1, retval___1, st_10))
-                              | _ => None
-                              end
-                            ) with
-                            | (Some (return___1, retval___1, st_10)) =>
-                              if return___1
-                              then (Some (retval___1, st_10))
-                              else (
-                                rely (((((test_PA v_0_Zptr).(meta_granule_offset)) mod (16)) = (0)));
-                                when st_14 == (
-                                    (granule_unlock_spec
-                                      (ret_record.(e_2))
-                                      ((st_10.[share].[globals].[g_granules] :<
-                                        ((((st_10.(share)).(globals)).(g_granules)) #
-                                          ((((test_PA v_0_Zptr).(meta_granule_offset)) + (4)) / (16)) ==
-                                          (((((st_10.(share)).(globals)).(g_granules)) @ ((((test_PA v_0_Zptr).(meta_granule_offset)) + (4)) / (16))).[e_state_s_granule] :< 5))).[share].[granule_data] :<
-                                        (((st_10.(share)).(granule_data)) #
-                                          ((((ret_record.(e_2)).(poffset)) + ((8 * ((ret_record.(e_3)))))) / (4096)) ==
-                                          ((((st_10.(share)).(granule_data)) @ ((((ret_record.(e_2)).(poffset)) + ((8 * ((ret_record.(e_3)))))) / (4096))).[g_norm] :<
-                                            (((((st_10.(share)).(granule_data)) @ ((((ret_record.(e_2)).(poffset)) + ((8 * ((ret_record.(e_3)))))) / (4096))).(g_norm)) #
-                                              ((((ret_record.(e_2)).(poffset)) + ((8 * ((ret_record.(e_3)))))) mod (4096)) ==
-                                              (test_PTE_Z (mkabs_PTE_t (test_PA v_0_Zptr) 3 0))))))));
-                                when st_15 == ((granule_unlock_spec (mkPtr "granules" ((test_PA v_0_Zptr).(meta_granule_offset))) st_14));
-                                (Some (0, st_15)))
-                            | None => None
-                            end)
-                          else (
-                            rely (((((test_PA v_0_Zptr).(meta_granule_offset)) mod (16)) = (0)));
-                            when st_14 == (
-                                (granule_unlock_spec
-                                  (ret_record.(e_2))
-                                  ((st_4.[share].[globals].[g_granules] :<
-                                    ((((st_4.(share)).(globals)).(g_granules)) #
-                                      ((((test_PA v_0_Zptr).(meta_granule_offset)) + (4)) / (16)) ==
-                                      (((((st_4.(share)).(globals)).(g_granules)) @ ((((test_PA v_0_Zptr).(meta_granule_offset)) + (4)) / (16))).[e_state_s_granule] :< 5))).[share].[granule_data] :<
-                                    (((st_4.(share)).(granule_data)) #
-                                      ((((ret_record.(e_2)).(poffset)) + ((8 * ((ret_record.(e_3)))))) / (4096)) ==
-                                      ((((st_4.(share)).(granule_data)) @ ((((ret_record.(e_2)).(poffset)) + ((8 * ((ret_record.(e_3)))))) / (4096))).[g_norm] :<
-                                        (((((st_4.(share)).(granule_data)) @ ((((ret_record.(e_2)).(poffset)) + ((8 * ((ret_record.(e_3)))))) / (4096))).(g_norm)) #
-                                          ((((ret_record.(e_2)).(poffset)) + ((8 * ((ret_record.(e_3)))))) mod (4096)) ==
-                                          (test_PTE_Z (mkabs_PTE_t (test_PA v_0_Zptr) 3 0))))))));
-                            when st_15 == ((granule_unlock_spec (mkPtr "granules" ((test_PA v_0_Zptr).(meta_granule_offset))) st_14));
-                            (Some (0, st_15)))))
-                      else (
-                        when st_6 == ((granule_unlock_spec (ret_record.(e_2)) st_4));
-                        when st_7 == ((granule_unlock_spec (mkPtr "granules" ((test_PA v_0_Zptr).(meta_granule_offset))) st_6));
-                        (Some ((pack_struct_return_code_para (make_return_code_para 8)), st_7))))
-                    else (Some ((pack_struct_return_code_para (make_return_code_para 1)), st')));
-                (Some (((v_23 << (32)) >> (32)), st_1))));
-          (Some (v__1, st_1)))
+                      rely ((true = (true)));
+                      when st_16 == (
+                          (granule_unlock_spec
+                            (rtt_ret.(e_2))
+                            (st_3.[share].[granule_data] :<
+                              (((st_3.(share)).(granule_data)) #
+                                ((((rtt_ret.(e_2)).(poffset)) + ((8 * ((rtt_ret.(e_3)))))) / (4096)) ==
+                                ((((st_3.(share)).(granule_data)) @ ((((rtt_ret.(e_2)).(poffset)) + ((8 * ((rtt_ret.(e_3)))))) / (4096))).[g_norm] :<
+                                  (((((st_3.(share)).(granule_data)) @ ((((rtt_ret.(e_2)).(poffset)) + ((8 * ((rtt_ret.(e_3)))))) / (4096))).(g_norm)) #
+                                    ((((rtt_ret.(e_2)).(poffset)) + ((8 * ((rtt_ret.(e_3)))))) mod (4096)) ==
+                                    (test_PTE_Z
+                                      (mkabs_PTE_t
+                                        ((abs_tte_read (mkPtr "granule_data" (((rtt_ret.(e_2)).(poffset)) + ((8 * ((rtt_ret.(e_3))))))) st_3).(meta_PA))
+                                        ((abs_tte_read (mkPtr "granule_data" (((rtt_ret.(e_2)).(poffset)) + ((8 * ((rtt_ret.(e_3))))))) st_3).(meta_desc_type))
+                                        v_3
+                                        ((abs_tte_read (mkPtr "granule_data" (((rtt_ret.(e_2)).(poffset)) + ((8 * ((rtt_ret.(e_3))))))) st_3).(meta_mem_attr))))))))));
+                      (Some (0, st_16)))
+                    else (
+                      when st_13 == ((granule_unlock_spec (rtt_ret.(e_2)) st_3));
+                      (Some ((pack_struct_return_code_para (make_return_code_para 8)), st_13))))))))
+          else (
+            when st_7 == ((granule_unlock_spec (rtt_ret.(e_2)) st_3));
+            (Some ((pack_struct_return_code_para (make_return_code_para 8)), st_7))))
         else (
-          when v_8, st_0 == (
-              when ret, st' == ((granule_try_lock_spec (mkPtr "granules" (((test_PA v_1_Zptr) & ((- 2))).(meta_granule_offset))) 3 st));
-              if ret
-              then (Some ((mkPtr "granules" (((test_PA v_1_Zptr) & ((- 2))).(meta_granule_offset))), st'))
-              else (Some ((mkPtr "null" 0), st')));
-          rely (((((v_8.(poffset)) mod (16)) = (0)) /\ (((v_8.(poffset)) >= (0)))));
-          rely ((((v_8.(pbase)) = ("granules")) \/ (((v_8.(pbase)) = ("null")))));
-          when v__1, st_1 == (
-              if (((v_8.(pbase)) =? ("null")) /\ (((v_8.(poffset)) =? (0))))
-              then (Some ((pack_struct_return_code_para (make_return_code_para 1)), st_0))
+          when st_2 == ((spinlock_release_spec (mkPtr "granules" ((test_PA v_0).(meta_granule_offset))) st_1));
+          (Some ((pack_struct_return_code_para (make_return_code_para 1)), st_2))))
+      else (
+        when st_1 == ((spinlock_acquire_spec (mkPtr "granules" ((test_PA v_0).(meta_granule_offset))) st));
+        if (((((((st_1.(share)).(globals)).(g_granules)) @ (((test_PA v_0).(meta_granule_offset)) / (16))).(e_state_s_granule)) - (3)) =? (0))
+        then (
+          rely ((((((test_PA v_0).(meta_granule_offset)) mod (16)) = (0)) /\ ((((test_PA v_0).(meta_granule_offset)) >= (0)))));
+          when st_4 == ((granule_lock_spec (rec_to_ttbr1_para (mkPtr "granule_data" ((test_PA v_0).(meta_granule_offset))) st_1) 5 st_1));
+          when st_5 == ((granule_unlock_spec (mkPtr "granules" ((test_PA v_0).(meta_granule_offset))) st_4));
+          when ret_rtt, st_7 == (
+              (rtt_walk_lock_unlock_spec_abs
+                (mkPtr "stack_s_rtt_walk" 0)
+                (rec_to_ttbr1_para (mkPtr "granule_data" ((test_PA v_0).(meta_granule_offset))) st_1)
+                0
+                64
+                v_1
+                v_2
+                st_5));
+          rely ((((st_7.(share)).(granule_data)) = (((st_5.(share)).(granule_data)))));
+          if (((ret_rtt.(e_1)) - (v_2)) =? (0))
+          then (
+            if ((v_2 <? (3)) && ((((abs_tte_read (mkPtr "granule_data" (((ret_rtt.(e_2)).(poffset)) + ((8 * ((ret_rtt.(e_3))))))) st_7).(meta_desc_type)) =? (3))))
+            then (
+              when st_16 == ((granule_unlock_spec (ret_rtt.(e_2)) st_7));
+              (Some ((pack_struct_return_code_para (make_return_code_para 8)), st_16)))
+            else (
+              if ((v_2 =? (3)) && ((((abs_tte_read (mkPtr "granule_data" (((ret_rtt.(e_2)).(poffset)) + ((8 * ((ret_rtt.(e_3))))))) st_7).(meta_desc_type)) =? (3))))
+              then (
+                if (v_3 =? (0))
+                then (
+                  when st_19 == (
+                      (granule_unlock_spec
+                        (ret_rtt.(e_2))
+                        (st_7.[share].[granule_data] :<
+                          (((st_7.(share)).(granule_data)) #
+                            ((((ret_rtt.(e_2)).(poffset)) + ((8 * ((ret_rtt.(e_3)))))) / (4096)) ==
+                            ((((st_7.(share)).(granule_data)) @ ((((ret_rtt.(e_2)).(poffset)) + ((8 * ((ret_rtt.(e_3)))))) / (4096))).[g_norm] :<
+                              (((((st_7.(share)).(granule_data)) @ ((((ret_rtt.(e_2)).(poffset)) + ((8 * ((ret_rtt.(e_3)))))) / (4096))).(g_norm)) #
+                                ((((ret_rtt.(e_2)).(poffset)) + ((8 * ((ret_rtt.(e_3)))))) mod (4096)) ==
+                                (test_PTE_Z (mkabs_PTE_t ((abs_tte_read (mkPtr "granule_data" (((ret_rtt.(e_2)).(poffset)) + ((8 * ((ret_rtt.(e_3))))))) st_7).(meta_PA)) 0 0 1))))))));
+                  (Some (0, st_19)))
+                else (
+                  when st_19 == (
+                      (granule_unlock_spec
+                        (ret_rtt.(e_2))
+                        (st_7.[share].[granule_data] :<
+                          (((st_7.(share)).(granule_data)) #
+                            ((((ret_rtt.(e_2)).(poffset)) + ((8 * ((ret_rtt.(e_3)))))) / (4096)) ==
+                            ((((st_7.(share)).(granule_data)) @ ((((ret_rtt.(e_2)).(poffset)) + ((8 * ((ret_rtt.(e_3)))))) / (4096))).[g_norm] :<
+                              (((((st_7.(share)).(granule_data)) @ ((((ret_rtt.(e_2)).(poffset)) + ((8 * ((ret_rtt.(e_3)))))) / (4096))).(g_norm)) #
+                                ((((ret_rtt.(e_2)).(poffset)) + ((8 * ((ret_rtt.(e_3)))))) mod (4096)) ==
+                                (test_PTE_Z (abs_tte_read (mkPtr "granule_data" (((ret_rtt.(e_2)).(poffset)) + ((8 * ((ret_rtt.(e_3))))))) st_7))))))));
+                  (Some (0, st_19))))
               else (
-                when v_15, st_2 == (
-                    when st_2 == ((granule_lock_spec (rec_to_ttbr1_para (mkPtr "granule_data" (v_8.(poffset))) st_0) 5 st_0));
-                    when v_7, st_3 == (
-                        when ret, st' == ((granule_try_lock_spec (mkPtr "granules" ((test_PA v_0_Zptr).(meta_granule_offset))) 1 st_2));
-                        if ret
-                        then (
-                          when ret_record, st_4 == ((rtt_walk_lock_unlock_spec_abs (mkPtr "stack_s_rtt_walk" 0) (rec_to_ttbr1_para (mkPtr "granule_data" (v_8.(poffset))) st_0) 0 64 v_2 v_3 st'));
-                          rely ((((ret_record.(e_2)).(pbase)) =s ("granules")));
-                          rely (((((ret_record.(e_2)).(poffset)) mod (16)) = (0)));
-                          rely ((((ret_record.(e_1)) <= (3)) /\ (((ret_record.(e_1)) >= (0)))));
-                          if (((ret_record.(e_1)) - ((v_3 + ((- 1))))) =? (0))
-                          then (
-                            if (
-                              ((((abs_tte_read (mkPtr "granule_data" (((ret_record.(e_2)).(poffset)) + ((8 * ((ret_record.(e_3))))))) st_4).(meta_desc_type)) =? (0)) &&
-                                ((((abs_tte_read (mkPtr "granule_data" (((ret_record.(e_2)).(poffset)) + ((8 * ((ret_record.(e_3))))))) st_4).(meta_ripas)) =? (0)))))
-                            then (
-                              when st_10 == (
-                                  (s2tt_init_unassigned_spec
-                                    (mkPtr "granule_data" ((test_PA v_0_Zptr).(meta_granule_offset)))
-                                    ((abs_tte_read (mkPtr "granule_data" (((ret_record.(e_2)).(poffset)) + ((8 * ((ret_record.(e_3))))))) st_4).(meta_ripas))
-                                    st_4));
-                              rely ((((((ret_record.(e_2)).(poffset)) + (8)) mod (16)) = (8)));
-                              rely (((((test_PA v_0_Zptr).(meta_granule_offset)) mod (16)) = (0)));
-                              when st_16 == (
-                                  (granule_unlock_spec
-                                    (ret_record.(e_2))
-                                    ((st_10.[share].[globals].[g_granules] :<
-                                      (((((st_10.(share)).(globals)).(g_granules)) #
-                                        ((((ret_record.(e_2)).(poffset)) + (8)) / (16)) ==
-                                        (((((st_10.(share)).(globals)).(g_granules)) @ ((((ret_record.(e_2)).(poffset)) + (8)) / (16))).[e_ref] :<
-                                          ((((((st_10.(share)).(globals)).(g_granules)) @ ((((ret_record.(e_2)).(poffset)) + (8)) / (16))).(e_ref)).[e_u_anon_3_0] :<
-                                            (((((((st_10.(share)).(globals)).(g_granules)) @ ((((ret_record.(e_2)).(poffset)) + (8)) / (16))).(e_ref)).(e_u_anon_3_0)) + (1))))) #
-                                        ((((test_PA v_0_Zptr).(meta_granule_offset)) + (4)) / (16)) ==
-                                        ((((((st_10.(share)).(globals)).(g_granules)) #
-                                          ((((ret_record.(e_2)).(poffset)) + (8)) / (16)) ==
-                                          (((((st_10.(share)).(globals)).(g_granules)) @ ((((ret_record.(e_2)).(poffset)) + (8)) / (16))).[e_ref] :<
-                                            ((((((st_10.(share)).(globals)).(g_granules)) @ ((((ret_record.(e_2)).(poffset)) + (8)) / (16))).(e_ref)).[e_u_anon_3_0] :<
-                                              (((((((st_10.(share)).(globals)).(g_granules)) @ ((((ret_record.(e_2)).(poffset)) + (8)) / (16))).(e_ref)).(e_u_anon_3_0)) + (1))))) @ ((((test_PA v_0_Zptr).(meta_granule_offset)) + (4)) / (16))).[e_state_s_granule] :<
-                                          5))).[share].[granule_data] :<
-                                      (((st_10.(share)).(granule_data)) #
-                                        ((((ret_record.(e_2)).(poffset)) + ((8 * ((ret_record.(e_3)))))) / (4096)) ==
-                                        ((((st_10.(share)).(granule_data)) @ ((((ret_record.(e_2)).(poffset)) + ((8 * ((ret_record.(e_3)))))) / (4096))).[g_norm] :<
-                                          (((((st_10.(share)).(granule_data)) @ ((((ret_record.(e_2)).(poffset)) + ((8 * ((ret_record.(e_3)))))) / (4096))).(g_norm)) #
-                                            ((((ret_record.(e_2)).(poffset)) + ((8 * ((ret_record.(e_3)))))) mod (4096)) ==
-                                            (test_PTE_Z (mkabs_PTE_t (test_PA v_0_Zptr) 3 0))))))));
-                              when st_17 == ((granule_unlock_spec (mkPtr "granules" ((test_PA v_0_Zptr).(meta_granule_offset))) st_16));
-                              (Some (0, st_17)))
-                            else (
-                              if (((v_3 + ((- 1))) <? (3)) && ((((abs_tte_read (mkPtr "granule_data" (((ret_record.(e_2)).(poffset)) + ((8 * ((ret_record.(e_3))))))) st_4).(meta_desc_type)) =? (3))))
-                              then (
-                                match (
-                                  match (
-                                    when st_11 == ((granule_unlock_spec (ret_record.(e_2)) st_4));
-                                    when st_12 == ((granule_unlock_spec (mkPtr "granules" ((test_PA v_0_Zptr).(meta_granule_offset))) st_11));
-                                    (Some (true, (pack_struct_return_code_para (make_return_code_para 9)), st_12))
-                                  ) with
-                                  | (Some (return___1, retval___1, st_10)) => (Some (return___1, retval___1, st_10))
-                                  | _ => None
-                                  end
-                                ) with
-                                | (Some (return___1, retval___1, st_10)) =>
-                                  if return___1
-                                  then (Some (retval___1, st_10))
-                                  else (
-                                    rely (((((test_PA v_0_Zptr).(meta_granule_offset)) mod (16)) = (0)));
-                                    when st_14 == (
-                                        (granule_unlock_spec
-                                          (ret_record.(e_2))
-                                          ((st_10.[share].[globals].[g_granules] :<
-                                            ((((st_10.(share)).(globals)).(g_granules)) #
-                                              ((((test_PA v_0_Zptr).(meta_granule_offset)) + (4)) / (16)) ==
-                                              (((((st_10.(share)).(globals)).(g_granules)) @ ((((test_PA v_0_Zptr).(meta_granule_offset)) + (4)) / (16))).[e_state_s_granule] :< 5))).[share].[granule_data] :<
-                                            (((st_10.(share)).(granule_data)) #
-                                              ((((ret_record.(e_2)).(poffset)) + ((8 * ((ret_record.(e_3)))))) / (4096)) ==
-                                              ((((st_10.(share)).(granule_data)) @ ((((ret_record.(e_2)).(poffset)) + ((8 * ((ret_record.(e_3)))))) / (4096))).[g_norm] :<
-                                                (((((st_10.(share)).(granule_data)) @ ((((ret_record.(e_2)).(poffset)) + ((8 * ((ret_record.(e_3)))))) / (4096))).(g_norm)) #
-                                                  ((((ret_record.(e_2)).(poffset)) + ((8 * ((ret_record.(e_3)))))) mod (4096)) ==
-                                                  (test_PTE_Z (mkabs_PTE_t (test_PA v_0_Zptr) 3 0))))))));
-                                    when st_15 == ((granule_unlock_spec (mkPtr "granules" ((test_PA v_0_Zptr).(meta_granule_offset))) st_14));
-                                    (Some (0, st_15)))
-                                | None => None
-                                end)
-                              else (
-                                rely (((((test_PA v_0_Zptr).(meta_granule_offset)) mod (16)) = (0)));
-                                when st_14 == (
-                                    (granule_unlock_spec
-                                      (ret_record.(e_2))
-                                      ((st_4.[share].[globals].[g_granules] :<
-                                        ((((st_4.(share)).(globals)).(g_granules)) #
-                                          ((((test_PA v_0_Zptr).(meta_granule_offset)) + (4)) / (16)) ==
-                                          (((((st_4.(share)).(globals)).(g_granules)) @ ((((test_PA v_0_Zptr).(meta_granule_offset)) + (4)) / (16))).[e_state_s_granule] :< 5))).[share].[granule_data] :<
-                                        (((st_4.(share)).(granule_data)) #
-                                          ((((ret_record.(e_2)).(poffset)) + ((8 * ((ret_record.(e_3)))))) / (4096)) ==
-                                          ((((st_4.(share)).(granule_data)) @ ((((ret_record.(e_2)).(poffset)) + ((8 * ((ret_record.(e_3)))))) / (4096))).[g_norm] :<
-                                            (((((st_4.(share)).(granule_data)) @ ((((ret_record.(e_2)).(poffset)) + ((8 * ((ret_record.(e_3)))))) / (4096))).(g_norm)) #
-                                              ((((ret_record.(e_2)).(poffset)) + ((8 * ((ret_record.(e_3)))))) mod (4096)) ==
-                                              (test_PTE_Z (mkabs_PTE_t (test_PA v_0_Zptr) 3 0))))))));
-                                when st_15 == ((granule_unlock_spec (mkPtr "granules" ((test_PA v_0_Zptr).(meta_granule_offset))) st_14));
-                                (Some (0, st_15)))))
-                          else (
-                            if (((ret_record.(e_1)) - (v_3)) =? (0))
-                            then (
-                              match (
-                                match (
-                                  match (
-                                    when st_6 == ((granule_unlock_spec (ret_record.(e_2)) st_4));
-                                    when st_7 == ((granule_unlock_spec (mkPtr "granules" ((test_PA v_0_Zptr).(meta_granule_offset))) st_6));
-                                    (Some (true, (pack_struct_return_code_para (make_return_code_para 9)), st_7))
-                                  ) with
-                                  | (Some (__return___0, __retval___0, st_5)) => (Some (__return___0, __retval___0, st_5))
-                                  | _ => None
-                                  end
-                                ) with
-                                | (Some (__return___0, __retval___0, st_5)) =>
-                                  if __return___0
-                                  then (Some (true, __retval___0, st_5))
-                                  else (
-                                    when st_7 == ((granule_unlock_spec (ret_record.(e_2)) st_5));
-                                    when st_8 == ((granule_unlock_spec (mkPtr "granules" ((test_PA v_0_Zptr).(meta_granule_offset))) st_7));
-                                    (Some (true, (pack_struct_return_code_para (make_return_code_para 8)), st_8)))
-                                | _ => None
-                                end
-                              ) with
-                              | (Some (__return___0, __retval___0, st_5)) =>
-                                if __return___0
-                                then (Some (__retval___0, st_5))
-                                else (
-                                  if (
-                                    ((((abs_tte_read (mkPtr "granule_data" (((ret_record.(e_2)).(poffset)) + ((8 * ((ret_record.(e_3))))))) st_5).(meta_desc_type)) =? (0)) &&
-                                      ((((abs_tte_read (mkPtr "granule_data" (((ret_record.(e_2)).(poffset)) + ((8 * ((ret_record.(e_3))))))) st_5).(meta_ripas)) =? (0)))))
-                                  then (
-                                    when st_11 == (
-                                        (s2tt_init_unassigned_spec
-                                          (mkPtr "granule_data" ((test_PA v_0_Zptr).(meta_granule_offset)))
-                                          ((abs_tte_read (mkPtr "granule_data" (((ret_record.(e_2)).(poffset)) + ((8 * ((ret_record.(e_3))))))) st_5).(meta_ripas))
-                                          st_5));
-                                    rely ((((((ret_record.(e_2)).(poffset)) + (8)) mod (16)) = (8)));
-                                    rely (((((test_PA v_0_Zptr).(meta_granule_offset)) mod (16)) = (0)));
-                                    when st_17 == (
-                                        (granule_unlock_spec
-                                          (ret_record.(e_2))
-                                          ((st_11.[share].[globals].[g_granules] :<
-                                            (((((st_11.(share)).(globals)).(g_granules)) #
-                                              ((((ret_record.(e_2)).(poffset)) + (8)) / (16)) ==
-                                              (((((st_11.(share)).(globals)).(g_granules)) @ ((((ret_record.(e_2)).(poffset)) + (8)) / (16))).[e_ref] :<
-                                                ((((((st_11.(share)).(globals)).(g_granules)) @ ((((ret_record.(e_2)).(poffset)) + (8)) / (16))).(e_ref)).[e_u_anon_3_0] :<
-                                                  (((((((st_11.(share)).(globals)).(g_granules)) @ ((((ret_record.(e_2)).(poffset)) + (8)) / (16))).(e_ref)).(e_u_anon_3_0)) + (1))))) #
-                                              ((((test_PA v_0_Zptr).(meta_granule_offset)) + (4)) / (16)) ==
-                                              ((((((st_11.(share)).(globals)).(g_granules)) #
-                                                ((((ret_record.(e_2)).(poffset)) + (8)) / (16)) ==
-                                                (((((st_11.(share)).(globals)).(g_granules)) @ ((((ret_record.(e_2)).(poffset)) + (8)) / (16))).[e_ref] :<
-                                                  ((((((st_11.(share)).(globals)).(g_granules)) @ ((((ret_record.(e_2)).(poffset)) + (8)) / (16))).(e_ref)).[e_u_anon_3_0] :<
-                                                    (((((((st_11.(share)).(globals)).(g_granules)) @ ((((ret_record.(e_2)).(poffset)) + (8)) / (16))).(e_ref)).(e_u_anon_3_0)) + (1))))) @ ((((test_PA v_0_Zptr).(meta_granule_offset)) + (4)) / (16))).[e_state_s_granule] :<
-                                                5))).[share].[granule_data] :<
-                                            (((st_11.(share)).(granule_data)) #
-                                              ((((ret_record.(e_2)).(poffset)) + ((8 * ((ret_record.(e_3)))))) / (4096)) ==
-                                              ((((st_11.(share)).(granule_data)) @ ((((ret_record.(e_2)).(poffset)) + ((8 * ((ret_record.(e_3)))))) / (4096))).[g_norm] :<
-                                                (((((st_11.(share)).(granule_data)) @ ((((ret_record.(e_2)).(poffset)) + ((8 * ((ret_record.(e_3)))))) / (4096))).(g_norm)) #
-                                                  ((((ret_record.(e_2)).(poffset)) + ((8 * ((ret_record.(e_3)))))) mod (4096)) ==
-                                                  (test_PTE_Z (mkabs_PTE_t (test_PA v_0_Zptr) 3 0))))))));
-                                    when st_18 == ((granule_unlock_spec (mkPtr "granules" ((test_PA v_0_Zptr).(meta_granule_offset))) st_17));
-                                    (Some (0, st_18)))
-                                  else (
-                                    if (((abs_tte_read (mkPtr "granule_data" (((ret_record.(e_2)).(poffset)) + ((8 * ((ret_record.(e_3))))))) st_5).(meta_desc_type)) =? (3))
-                                    then (
-                                      match (
-                                        match (
-                                          when st_12 == ((granule_unlock_spec (ret_record.(e_2)) st_5));
-                                          when st_13 == ((granule_unlock_spec (mkPtr "granules" ((test_PA v_0_Zptr).(meta_granule_offset))) st_12));
-                                          (Some (true, (pack_struct_return_code_para (make_return_code_para 9)), st_13))
-                                        ) with
-                                        | (Some (return___1, retval___1, st_11)) => (Some (return___1, retval___1, st_11))
-                                        | _ => None
-                                        end
-                                      ) with
-                                      | (Some (return___1, retval___1, st_11)) =>
-                                        if return___1
-                                        then (Some (retval___1, st_11))
-                                        else (
-                                          rely (((((test_PA v_0_Zptr).(meta_granule_offset)) mod (16)) = (0)));
-                                          when st_15 == (
-                                              (granule_unlock_spec
-                                                (ret_record.(e_2))
-                                                ((st_11.[share].[globals].[g_granules] :<
-                                                  ((((st_11.(share)).(globals)).(g_granules)) #
-                                                    ((((test_PA v_0_Zptr).(meta_granule_offset)) + (4)) / (16)) ==
-                                                    (((((st_11.(share)).(globals)).(g_granules)) @ ((((test_PA v_0_Zptr).(meta_granule_offset)) + (4)) / (16))).[e_state_s_granule] :< 5))).[share].[granule_data] :<
-                                                  (((st_11.(share)).(granule_data)) #
-                                                    ((((ret_record.(e_2)).(poffset)) + ((8 * ((ret_record.(e_3)))))) / (4096)) ==
-                                                    ((((st_11.(share)).(granule_data)) @ ((((ret_record.(e_2)).(poffset)) + ((8 * ((ret_record.(e_3)))))) / (4096))).[g_norm] :<
-                                                      (((((st_11.(share)).(granule_data)) @ ((((ret_record.(e_2)).(poffset)) + ((8 * ((ret_record.(e_3)))))) / (4096))).(g_norm)) #
-                                                        ((((ret_record.(e_2)).(poffset)) + ((8 * ((ret_record.(e_3)))))) mod (4096)) ==
-                                                        (test_PTE_Z (mkabs_PTE_t (test_PA v_0_Zptr) 3 0))))))));
-                                          when st_16 == ((granule_unlock_spec (mkPtr "granules" ((test_PA v_0_Zptr).(meta_granule_offset))) st_15));
-                                          (Some (0, st_16)))
-                                      | None => None
-                                      end)
-                                    else (
-                                      rely (((((test_PA v_0_Zptr).(meta_granule_offset)) mod (16)) = (0)));
-                                      when st_15 == (
-                                          (granule_unlock_spec
-                                            (ret_record.(e_2))
-                                            ((st_5.[share].[globals].[g_granules] :<
-                                              ((((st_5.(share)).(globals)).(g_granules)) #
-                                                ((((test_PA v_0_Zptr).(meta_granule_offset)) + (4)) / (16)) ==
-                                                (((((st_5.(share)).(globals)).(g_granules)) @ ((((test_PA v_0_Zptr).(meta_granule_offset)) + (4)) / (16))).[e_state_s_granule] :< 5))).[share].[granule_data] :<
-                                              (((st_5.(share)).(granule_data)) #
-                                                ((((ret_record.(e_2)).(poffset)) + ((8 * ((ret_record.(e_3)))))) / (4096)) ==
-                                                ((((st_5.(share)).(granule_data)) @ ((((ret_record.(e_2)).(poffset)) + ((8 * ((ret_record.(e_3)))))) / (4096))).[g_norm] :<
-                                                  (((((st_5.(share)).(granule_data)) @ ((((ret_record.(e_2)).(poffset)) + ((8 * ((ret_record.(e_3)))))) / (4096))).(g_norm)) #
-                                                    ((((ret_record.(e_2)).(poffset)) + ((8 * ((ret_record.(e_3)))))) mod (4096)) ==
-                                                    (test_PTE_Z (mkabs_PTE_t (test_PA v_0_Zptr) 3 0))))))));
-                                      when st_16 == ((granule_unlock_spec (mkPtr "granules" ((test_PA v_0_Zptr).(meta_granule_offset))) st_15));
-                                      (Some (0, st_16)))))
-                              | None => None
-                              end)
-                            else (
-                              when st_7 == ((granule_unlock_spec (ret_record.(e_2)) st_4));
-                              when st_8 == ((granule_unlock_spec (mkPtr "granules" ((test_PA v_0_Zptr).(meta_granule_offset))) st_7));
-                              (Some ((pack_struct_return_code_para (make_return_code_para 8)), st_8)))))
-                        else (Some ((pack_struct_return_code_para (make_return_code_para 1)), st')));
-                    ((Some v_7), st_3));
-                when st_3 == ((granule_unlock_spec v_8 st_2));
-                (Some (((v_15 << (32)) >> (32)), st_3))));
-          (Some (v__1, st_1))));
-    (Some (v__0, st_0)).
+                if ((v_2 <>? (3)) && ((((abs_tte_read (mkPtr "granule_data" (((ret_rtt.(e_2)).(poffset)) + ((8 * ((ret_rtt.(e_3))))))) st_7).(meta_desc_type)) =? (1))))
+                then (
+                  if (v_3 =? (0))
+                  then (
+                    rely ((true = (true)));
+                    when st_19 == (
+                        (granule_unlock_spec
+                          (ret_rtt.(e_2))
+                          (st_7.[share].[granule_data] :<
+                            (((st_7.(share)).(granule_data)) #
+                              ((((ret_rtt.(e_2)).(poffset)) + ((8 * ((ret_rtt.(e_3)))))) / (4096)) ==
+                              ((((st_7.(share)).(granule_data)) @ ((((ret_rtt.(e_2)).(poffset)) + ((8 * ((ret_rtt.(e_3)))))) / (4096))).[g_norm] :<
+                                (((((st_7.(share)).(granule_data)) @ ((((ret_rtt.(e_2)).(poffset)) + ((8 * ((ret_rtt.(e_3)))))) / (4096))).(g_norm)) #
+                                  ((((ret_rtt.(e_2)).(poffset)) + ((8 * ((ret_rtt.(e_3)))))) mod (4096)) ==
+                                  (test_PTE_Z (mkabs_PTE_t ((abs_tte_read (mkPtr "granule_data" (((ret_rtt.(e_2)).(poffset)) + ((8 * ((ret_rtt.(e_3))))))) st_7).(meta_PA)) 0 0 1))))))));
+                    (Some (0, st_19)))
+                  else (
+                    rely ((true = (true)));
+                    when st_19 == (
+                        (granule_unlock_spec
+                          (ret_rtt.(e_2))
+                          (st_7.[share].[granule_data] :<
+                            (((st_7.(share)).(granule_data)) #
+                              ((((ret_rtt.(e_2)).(poffset)) + ((8 * ((ret_rtt.(e_3)))))) / (4096)) ==
+                              ((((st_7.(share)).(granule_data)) @ ((((ret_rtt.(e_2)).(poffset)) + ((8 * ((ret_rtt.(e_3)))))) / (4096))).[g_norm] :<
+                                (((((st_7.(share)).(granule_data)) @ ((((ret_rtt.(e_2)).(poffset)) + ((8 * ((ret_rtt.(e_3)))))) / (4096))).(g_norm)) #
+                                  ((((ret_rtt.(e_2)).(poffset)) + ((8 * ((ret_rtt.(e_3)))))) mod (4096)) ==
+                                  (test_PTE_Z (abs_tte_read (mkPtr "granule_data" (((ret_rtt.(e_2)).(poffset)) + ((8 * ((ret_rtt.(e_3))))))) st_7))))))));
+                    (Some (0, st_19))))
+                else (
+                  if (
+                    (((((abs_tte_read (mkPtr "granule_data" (((ret_rtt.(e_2)).(poffset)) + ((8 * ((ret_rtt.(e_3))))))) st_7).(meta_desc_type)) =? (0)) &&
+                      ((((abs_tte_read (mkPtr "granule_data" (((ret_rtt.(e_2)).(poffset)) + ((8 * ((ret_rtt.(e_3))))))) st_7).(meta_ripas)) =? (0)))) &&
+                      ((((abs_tte_read (mkPtr "granule_data" (((ret_rtt.(e_2)).(poffset)) + ((8 * ((ret_rtt.(e_3))))))) st_7).(meta_mem_attr)) =? (0)))))
+                  then (
+                    when st_19 == (
+                        (granule_unlock_spec
+                          (ret_rtt.(e_2))
+                          (st_7.[share].[granule_data] :<
+                            (((st_7.(share)).(granule_data)) #
+                              ((((ret_rtt.(e_2)).(poffset)) + ((8 * ((ret_rtt.(e_3)))))) / (4096)) ==
+                              ((((st_7.(share)).(granule_data)) @ ((((ret_rtt.(e_2)).(poffset)) + ((8 * ((ret_rtt.(e_3)))))) / (4096))).[g_norm] :<
+                                (((((st_7.(share)).(granule_data)) @ ((((ret_rtt.(e_2)).(poffset)) + ((8 * ((ret_rtt.(e_3)))))) / (4096))).(g_norm)) #
+                                  ((((ret_rtt.(e_2)).(poffset)) + ((8 * ((ret_rtt.(e_3)))))) mod (4096)) ==
+                                  (test_PTE_Z
+                                    (mkabs_PTE_t
+                                      ((abs_tte_read (mkPtr "granule_data" (((ret_rtt.(e_2)).(poffset)) + ((8 * ((ret_rtt.(e_3))))))) st_7).(meta_PA))
+                                      ((abs_tte_read (mkPtr "granule_data" (((ret_rtt.(e_2)).(poffset)) + ((8 * ((ret_rtt.(e_3))))))) st_7).(meta_desc_type))
+                                      v_3
+                                      ((abs_tte_read (mkPtr "granule_data" (((ret_rtt.(e_2)).(poffset)) + ((8 * ((ret_rtt.(e_3))))))) st_7).(meta_mem_attr))))))))));
+                    (Some (0, st_19)))
+                  else (
+                    if (
+                      (((((abs_tte_read (mkPtr "granule_data" (((ret_rtt.(e_2)).(poffset)) + ((8 * ((ret_rtt.(e_3))))))) st_7).(meta_desc_type)) =? (0)) &&
+                        ((((abs_tte_read (mkPtr "granule_data" (((ret_rtt.(e_2)).(poffset)) + ((8 * ((ret_rtt.(e_3))))))) st_7).(meta_ripas)) =? (0)))) &&
+                        ((((abs_tte_read (mkPtr "granule_data" (((ret_rtt.(e_2)).(poffset)) + ((8 * ((ret_rtt.(e_3))))))) st_7).(meta_mem_attr)) =? (1)))))
+                    then (
+                      rely ((true = (true)));
+                      when st_19 == (
+                          (granule_unlock_spec
+                            (ret_rtt.(e_2))
+                            (st_7.[share].[granule_data] :<
+                              (((st_7.(share)).(granule_data)) #
+                                ((((ret_rtt.(e_2)).(poffset)) + ((8 * ((ret_rtt.(e_3)))))) / (4096)) ==
+                                ((((st_7.(share)).(granule_data)) @ ((((ret_rtt.(e_2)).(poffset)) + ((8 * ((ret_rtt.(e_3)))))) / (4096))).[g_norm] :<
+                                  (((((st_7.(share)).(granule_data)) @ ((((ret_rtt.(e_2)).(poffset)) + ((8 * ((ret_rtt.(e_3)))))) / (4096))).(g_norm)) #
+                                    ((((ret_rtt.(e_2)).(poffset)) + ((8 * ((ret_rtt.(e_3)))))) mod (4096)) ==
+                                    (test_PTE_Z
+                                      (mkabs_PTE_t
+                                        ((abs_tte_read (mkPtr "granule_data" (((ret_rtt.(e_2)).(poffset)) + ((8 * ((ret_rtt.(e_3))))))) st_7).(meta_PA))
+                                        ((abs_tte_read (mkPtr "granule_data" (((ret_rtt.(e_2)).(poffset)) + ((8 * ((ret_rtt.(e_3))))))) st_7).(meta_desc_type))
+                                        v_3
+                                        ((abs_tte_read (mkPtr "granule_data" (((ret_rtt.(e_2)).(poffset)) + ((8 * ((ret_rtt.(e_3))))))) st_7).(meta_mem_attr))))))))));
+                      (Some (0, st_19)))
+                    else (
+                      when st_16 == ((granule_unlock_spec (ret_rtt.(e_2)) st_7));
+                      (Some ((pack_struct_return_code_para (make_return_code_para 8)), st_16))))))))
+          else (
+            when st_11 == ((granule_unlock_spec (ret_rtt.(e_2)) st_7));
+            (Some ((pack_struct_return_code_para (make_return_code_para 8)), st_11))))
+        else (
+          when st_2 == ((spinlock_release_spec (mkPtr "granules" ((test_PA v_0).(meta_granule_offset))) st_1));
+          (Some ((pack_struct_return_code_para (make_return_code_para 1)), st_2))))).
 
 End Layer9_Spec.
 
-#[global] Hint Unfold rsi_rtt_create_spec: spec.
+#[global] Hint Unfold map_unmap_ns_s1_0_low: spec.
+#[global] Hint Unfold map_unmap_ns_s1_1_low: spec.
+#[global] Hint Unfold map_unmap_ns_s1_2_low: spec.
+#[global] Hint Unfold map_unmap_ns_s1_3_low: spec.
+#[global] Hint Unfold rsi_rtt_set_ripas_0: spec.
+#[global] Hint Unfold rsi_rtt_set_ripas_1: spec.
+#[global] Hint Unfold rsi_rtt_set_ripas_spec: spec.
