container/coq/pointer/.CachedSpec/Layer5Spec.v
@@ -7,7 +7,7 @@ Parameter memcpy_ns_read_spec_state_oracle : Ptr -> (Ptr -> (Z -> (RData -> (opt
 Parameter monitor_call_state_oracle : Z -> (Z -> (Z -> (Z -> (Z -> (Z -> (Z -> (RData -> (option (Z * RData))))))))).
 
 Definition s2tte_create_unassigned_spec_abs (v_0: Z) (st: RData) : (option (abs_PTE_t * RData)) :=
-  (Some ((mkabs_PTE_t (mkabs_PA_t (- 1)) 0 v_0), st)).
+  (Some ((mkabs_PTE_t (mkabs_PA_t (- 1)) 0 v_0 0), st)).
 
 Definition llvm_memset_p0i8_i64_spec (v_0: Ptr) (arg1: Z) (arg2: Z) (arg3: bool) (st: RData) : (option RData) :=
   when st_0 == ((llvm_memset_p0i8_i64_spec_state_oracle v_0 arg1 arg2 arg3 st));
@@ -51,6 +51,9 @@ Definition atomic_add_64 (loc: Ptr) (val: Z) (st: RData) : (option RData) :=
   when st_2 == ((store_RData_granules 64 loc (v + (val)) st_1));
   (Some st_2).
 
+Definition s2tte_is_table_spec (v_0: Z) (v_1: Z) (st: RData) : (option (bool * RData)) :=
+  (Some (((v_1 <? (3)) && (((v_0 & (3)) =? (3)))), st)).
+
 Definition granule_unlock_spec (v_0: Ptr) (st: RData) : (option RData) :=
   when st_0 == ((spinlock_release_spec (mkPtr (v_0.(pbase)) (v_0.(poffset))) st));
   (Some st_0).
@@ -78,31 +81,6 @@ Definition pack_struct_return_code_spec (v_0: Z) (st: RData) : (option (Z * RDat
 Definition make_return_code_spec (v_0: Z) (v_1: Z) (st: RData) : (option (Z * RData)) :=
   (Some ((make_return_code_para v_0), st)).
 
-Definition atomic_granule_get_spec (v_0: Ptr) (st: RData) : (option RData) :=
-  rely (((v_0.(pbase)) =s ("granules")));
-  rely (((((v_0.(poffset)) + (8)) mod (16)) = (8)));
-  (Some (st.[share].[globals].[g_granules] :<
-    ((((st.(share)).(globals)).(g_granules)) #
-      (((v_0.(poffset)) + (8)) / (16)) ==
-      (((((st.(share)).(globals)).(g_granules)) @ (((v_0.(poffset)) + (8)) / (16))).[e_ref] :<
-        ((((((st.(share)).(globals)).(g_granules)) @ (((v_0.(poffset)) + (8)) / (16))).(e_ref)).[e_u_anon_3_0] :<
-          (((((((st.(share)).(globals)).(g_granules)) @ (((v_0.(poffset)) + (8)) / (16))).(e_ref)).(e_u_anon_3_0)) + (1))))))).
-
-Definition atomic_granule_put_spec (v_0: Ptr) (st: RData) : (option RData) :=
-  rely (((v_0.(pbase)) =s ("granules")));
-  rely (((((v_0.(poffset)) + (8)) mod (16)) = (8)));
-  (Some (st.[share].[globals].[g_granules] :<
-    ((((st.(share)).(globals)).(g_granules)) #
-      (((v_0.(poffset)) + (8)) / (16)) ==
-      (((((st.(share)).(globals)).(g_granules)) @ (((v_0.(poffset)) + (8)) / (16))).[e_ref] :<
-        ((((((st.(share)).(globals)).(g_granules)) @ (((v_0.(poffset)) + (8)) / (16))).(e_ref)).[e_u_anon_3_0] :<
-          (((((((st.(share)).(globals)).(g_granules)) @ (((v_0.(poffset)) + (8)) / (16))).(e_ref)).(e_u_anon_3_0)) + ((- 1)))))))).
-
 Definition find_lock_granule_spec (v_0: abs_PA_t) (v_1: Z) (st: RData) : (option (Ptr * RData)) :=
   None.
-
-Definition s2tte_create_unassigned_spec (v_0: Z) (st: RData) : (option (Z * RData)) :=
-  if (v_0 =? (0))
-  then (Some (0, st))
-  else (Some (64, st)).
 
