container/coq/pointer/.CachedSpec/Layer8Spec.v
@@ -1,4 +1,34 @@
+Parameter test_Ptr_PTE : Ptr -> abs_PTE_t.
+
 Parameter rec_to_ttbr1_para : Ptr -> (RData -> Ptr).
+
+Definition update_ripas_spec_abs (v_0: abs_PTE_t) (v_1: Z) (v_2: Z) (st: RData) : (option (bool * abs_PTE_t)) :=
+  when v_5, st_1 == ((s2tte_is_table_spec_abs v_0 v_1 st));
+  if v_5
+  then (Some (false, v_0))
+  else (
+    when v_9, st_2 == ((s1tte_is_valid_spec_abs v_0 v_1 st_1));
+    if v_9
+    then (
+      if (v_2 =? (0))
+      then (
+        when v_14, st_3 == ((s2tte_pa_spec_abs v_0 v_1 st_2));
+        when v_15, st_4 == ((s2tte_create_assigned_spec_abs v_14 v_1 st_3));
+        (Some (true, v_15)))
+      else (Some (true, v_0)))
+    else (
+      when v_19, st_5 == ((s2tte_is_unassigned_spec_abs v_0 st_1));
+      if v_19
+      then (
+        let v_with_ripas := (mkabs_PTE_t (v_0.(meta_PA)) (v_0.(meta_desc_type)) v_2 (v_0.(meta_mem_attr))) in
+        (Some (true, v_with_ripas)))
+      else (
+        when v_22, st_7 == ((s2tte_is_assigned_spec_abs v_0 v_1 st_5));
+        if v_22
+        then (
+          let v_with_ripas := (mkabs_PTE_t (v_0.(meta_PA)) (v_0.(meta_desc_type)) v_2 (v_0.(meta_mem_attr))) in
+          (Some (true, v_with_ripas)))
+        else (Some (false, v_0))))).
 
 Definition rtt_create_s1_el1_spec_abs (v_0: Ptr) (v_1: abs_PA_t) (v_2: Z) (v_3: Z) (st: RData) : (option (Z * RData)) :=
   let ttbr := (rec_to_ttbr1_para v_0 st) in
@@ -6,496 +36,20 @@ Definition rtt_create_s1_el1_spec_abs (v_0: Ptr) (v_1: abs_PA_t) (v_2: Z) (v_3: 
   when v_7, st_2 == ((rtt_create_internal_spec_abs ttbr v_1 v_2 v_3 1 st_1));
   ((Some v_7), st_2).
 
-Definition map_unmap_ns_s1_0 (st_0: RData) (st_12: RData) (v_17: Ptr) (v_3: abs_PTE_t) (v_31: Z) (v__sroa_0_0_copyload: Ptr) (v__sroa_7_0_copyload: Z) : (option (Z * RData)) :=
-  rely (((v_31 =? (0)) = (true)));
-  rely (((v__sroa_0_0_copyload.(pbase)) =s ("granules")));
-  rely (((((v__sroa_0_0_copyload.(poffset)) + (8)) mod (16)) = (8)));
-  when st_19 == (
-      (granule_unlock_spec
-        v__sroa_0_0_copyload
-        ((st_12.[share].[globals].[g_granules] :<
-          ((((st_12.(share)).(globals)).(g_granules)) #
-            (((v__sroa_0_0_copyload.(poffset)) + (8)) / (16)) ==
-            (((((st_12.(share)).(globals)).(g_granules)) @ (((v__sroa_0_0_copyload.(poffset)) + (8)) / (16))).[e_ref] :<
-              ((((((st_12.(share)).(globals)).(g_granules)) @ (((v__sroa_0_0_copyload.(poffset)) + (8)) / (16))).(e_ref)).[e_u_anon_3_0] :<
-                (((((((st_12.(share)).(globals)).(g_granules)) @ (((v__sroa_0_0_copyload.(poffset)) + (8)) / (16))).(e_ref)).(e_u_anon_3_0)) + (1)))))).[share].[granule_data] :<
-          (((st_12.(share)).(granule_data)) #
-            (((v_17.(poffset)) + ((8 * (v__sroa_7_0_copyload)))) / (4096)) ==
-            ((((st_12.(share)).(granule_data)) @ (((v_17.(poffset)) + ((8 * (v__sroa_7_0_copyload)))) / (4096))).[g_norm] :<
-              (((((st_12.(share)).(granule_data)) @ (((v_17.(poffset)) + ((8 * (v__sroa_7_0_copyload)))) / (4096))).(g_norm)) #
-                (((v_17.(poffset)) + ((8 * (v__sroa_7_0_copyload)))) mod (4096)) ==
-                (test_PTE_Z v_3)))))));
-  (Some (0, st_19)).
-
-Definition map_unmap_ns_s1_1 (st_0: RData) (st_11: RData) (v_17: Ptr) (v_3: abs_PTE_t) (v__sroa_0_0_copyload: Ptr) (v__sroa_7_0_copyload: Z) : (option (Z * RData)) :=
-  rely (((v__sroa_0_0_copyload.(pbase)) =s ("granules")));
-  rely (((((v__sroa_0_0_copyload.(poffset)) + (8)) mod (16)) = (8)));
-  when st_18 == (
-      (granule_unlock_spec
-        v__sroa_0_0_copyload
-        ((st_11.[share].[globals].[g_granules] :<
-          ((((st_11.(share)).(globals)).(g_granules)) #
-            (((v__sroa_0_0_copyload.(poffset)) + (8)) / (16)) ==
-            (((((st_11.(share)).(globals)).(g_granules)) @ (((v__sroa_0_0_copyload.(poffset)) + (8)) / (16))).[e_ref] :<
-              ((((((st_11.(share)).(globals)).(g_granules)) @ (((v__sroa_0_0_copyload.(poffset)) + (8)) / (16))).(e_ref)).[e_u_anon_3_0] :<
-                (((((((st_11.(share)).(globals)).(g_granules)) @ (((v__sroa_0_0_copyload.(poffset)) + (8)) / (16))).(e_ref)).(e_u_anon_3_0)) + (1)))))).[share].[granule_data] :<
-          (((st_11.(share)).(granule_data)) #
-            (((v_17.(poffset)) + ((8 * (v__sroa_7_0_copyload)))) / (4096)) ==
-            ((((st_11.(share)).(granule_data)) @ (((v_17.(poffset)) + ((8 * (v__sroa_7_0_copyload)))) / (4096))).[g_norm] :<
-              (((((st_11.(share)).(granule_data)) @ (((v_17.(poffset)) + ((8 * (v__sroa_7_0_copyload)))) / (4096))).(g_norm)) #
-                (((v_17.(poffset)) + ((8 * (v__sroa_7_0_copyload)))) mod (4096)) ==
-                (test_PTE_Z v_3)))))));
-  (Some (0, st_18)).
-
-Definition map_unmap_ns_s1_2 (st_0: RData) (st_12: RData) (v_17: Ptr) (v_47: Z) (v__sroa_0_0_copyload: Ptr) (v__sroa_7_0_copyload: Z) : (option (Z * RData)) :=
-  rely (((v_47 =? (0)) = (true)));
-  rely (((((v__sroa_0_0_copyload.(pbase)) = ("granules")) /\ ((((v__sroa_0_0_copyload.(poffset)) mod (16)) = (0)))) /\ (((v__sroa_0_0_copyload.(poffset)) >= (0)))));
-  when st_20 == (
-      (granule_unlock_spec
-        v__sroa_0_0_copyload
-        ((st_12.[share].[globals].[g_granules] :<
-          ((((st_12.(share)).(globals)).(g_granules)) #
-            ((v__sroa_0_0_copyload.(poffset)) / (16)) ==
-            (((((st_12.(share)).(globals)).(g_granules)) @ ((v__sroa_0_0_copyload.(poffset)) / (16))).[e_ref] :<
-              ((((((st_12.(share)).(globals)).(g_granules)) @ ((v__sroa_0_0_copyload.(poffset)) / (16))).(e_ref)).[e_u_anon_3_0] :<
-                (((((((st_12.(share)).(globals)).(g_granules)) @ ((v__sroa_0_0_copyload.(poffset)) / (16))).(e_ref)).(e_u_anon_3_0)) + ((- 1))))))).[share].[granule_data] :<
-          (((st_12.(share)).(granule_data)) #
-            (((v_17.(poffset)) + ((8 * (v__sroa_7_0_copyload)))) / (4096)) ==
-            ((((st_12.(share)).(granule_data)) @ (((v_17.(poffset)) + ((8 * (v__sroa_7_0_copyload)))) / (4096))).[g_norm] :<
-              (((((st_12.(share)).(granule_data)) @ (((v_17.(poffset)) + ((8 * (v__sroa_7_0_copyload)))) / (4096))).(g_norm)) #
-                (((v_17.(poffset)) + ((8 * (v__sroa_7_0_copyload)))) mod (4096)) ==
-                (test_PTE_Z (mkabs_PTE_t (mkabs_PA_t (- 1)) 0 1))))))));
-  (Some (0, st_20)).
-
-Definition map_unmap_ns_s1_3 (st_0: RData) (st_11: RData) (v_17: Ptr) (v_20: abs_PTE_t) (v__sroa_0_0_copyload: Ptr) (v__sroa_7_0_copyload: Z) : (option (Z * RData)) :=
-  rely (((((v__sroa_0_0_copyload.(pbase)) = ("granules")) /\ ((((v__sroa_0_0_copyload.(poffset)) mod (16)) = (0)))) /\ (((v__sroa_0_0_copyload.(poffset)) >= (0)))));
-  when st_19 == (
-      (granule_unlock_spec
-        v__sroa_0_0_copyload
-        ((st_11.[share].[globals].[g_granules] :<
-          ((((st_11.(share)).(globals)).(g_granules)) #
-            ((v__sroa_0_0_copyload.(poffset)) / (16)) ==
-            (((((st_11.(share)).(globals)).(g_granules)) @ ((v__sroa_0_0_copyload.(poffset)) / (16))).[e_ref] :<
-              ((((((st_11.(share)).(globals)).(g_granules)) @ ((v__sroa_0_0_copyload.(poffset)) / (16))).(e_ref)).[e_u_anon_3_0] :<
-                (((((((st_11.(share)).(globals)).(g_granules)) @ ((v__sroa_0_0_copyload.(poffset)) / (16))).(e_ref)).(e_u_anon_3_0)) + ((- 1))))))).[share].[granule_data] :<
-          (((st_11.(share)).(granule_data)) #
-            (((v_17.(poffset)) + ((8 * (v__sroa_7_0_copyload)))) / (4096)) ==
-            ((((st_11.(share)).(granule_data)) @ (((v_17.(poffset)) + ((8 * (v__sroa_7_0_copyload)))) / (4096))).[g_norm] :<
-              (((((st_11.(share)).(granule_data)) @ (((v_17.(poffset)) + ((8 * (v__sroa_7_0_copyload)))) / (4096))).(g_norm)) #
-                (((v_17.(poffset)) + ((8 * (v__sroa_7_0_copyload)))) mod (4096)) ==
-                (test_PTE_Z (mkabs_PTE_t (mkabs_PA_t (- 1)) 0 1))))))));
-  (Some (0, st_19)).
-
-Definition map_unmap_ns_s1_spec (v_0_Zptr: Z) (v_1: Z) (v_2: Z) (v_3: Z) (v_4: Z) (st: RData) : (option (Z * RData)) :=
-  when st_3 == ((granule_lock_spec (mkPtr "granules" ((test_PA v_0_Zptr).(meta_granule_offset))) 5 st));
-  when ret_rtt, st_4 == ((rtt_walk_lock_unlock_spec_abs (mkPtr "stack_s_rtt_walk" 0) (mkPtr "granules" ((test_PA v_0_Zptr).(meta_granule_offset))) 0 64 v_1 v_2 st_3));
-  rely ((((st_4.(share)).(granule_data)) = (((st_3.(share)).(granule_data)))));
-  if (((ret_rtt.(e_1)) - (v_2)) =? (0))
-  then (
-    if (v_4 =? (0))
-    then (
-      if (
-        ((((abs_tte_read (mkPtr "granule_data" (((ret_rtt.(e_2)).(poffset)) + ((8 * ((ret_rtt.(e_3))))))) st_4).(meta_desc_type)) =? (0)) &&
-          ((((abs_tte_read (mkPtr "granule_data" (((ret_rtt.(e_2)).(poffset)) + ((8 * ((ret_rtt.(e_3))))))) st_4).(meta_ripas)) =? (0)))))
-      then (
-        if (uart0_phys_para (test_Z_PTE v_3))
-        then (
-          rely ((((ret_rtt.(e_2)).(pbase)) =s ("granules")));
-          rely ((((((ret_rtt.(e_2)).(poffset)) + (8)) mod (16)) = (8)));
-          when st_18 == (
-              (granule_unlock_spec
-                (ret_rtt.(e_2))
-                ((st_4.[share].[globals].[g_granules] :<
-                  ((((st_4.(share)).(globals)).(g_granules)) #
-                    ((((ret_rtt.(e_2)).(poffset)) + (8)) / (16)) ==
-                    (((((st_4.(share)).(globals)).(g_granules)) @ ((((ret_rtt.(e_2)).(poffset)) + (8)) / (16))).[e_ref] :<
-                      ((((((st_4.(share)).(globals)).(g_granules)) @ ((((ret_rtt.(e_2)).(poffset)) + (8)) / (16))).(e_ref)).[e_u_anon_3_0] :<
-                        (((((((st_4.(share)).(globals)).(g_granules)) @ ((((ret_rtt.(e_2)).(poffset)) + (8)) / (16))).(e_ref)).(e_u_anon_3_0)) + (1)))))).[share].[granule_data] :<
-                  (((st_4.(share)).(granule_data)) #
-                    ((((ret_rtt.(e_2)).(poffset)) + ((8 * ((ret_rtt.(e_3)))))) / (4096)) ==
-                    ((((st_4.(share)).(granule_data)) @ ((((ret_rtt.(e_2)).(poffset)) + ((8 * ((ret_rtt.(e_3)))))) / (4096))).[g_norm] :<
-                      (((((st_4.(share)).(granule_data)) @ ((((ret_rtt.(e_2)).(poffset)) + ((8 * ((ret_rtt.(e_3)))))) / (4096))).(g_norm)) #
-                        ((((ret_rtt.(e_2)).(poffset)) + ((8 * ((ret_rtt.(e_3)))))) mod (4096)) ==
-                        (test_PTE_Z (test_Z_PTE v_3))))))));
-          (Some (0, st_18)))
-        else (
-          when st_1 == ((spinlock_acquire_spec (mkPtr "granules" (((test_Z_PTE v_3).(meta_PA)).(meta_granule_offset))) st_4));
-          if ((((((st_1.(share)).(globals)).(g_granules)) @ ((((test_Z_PTE v_3).(meta_PA)).(meta_granule_offset)) / (16))).(e_state_s_granule)) =? (0))
-          then (
-            rely (((((((test_Z_PTE v_3).(meta_PA)).(meta_granule_offset)) mod (16)) = (0)) /\ (((((test_Z_PTE v_3).(meta_PA)).(meta_granule_offset)) >= (0)))));
-            when st_6 == (
-                (granule_unlock_spec
-                  (mkPtr "granules" (((test_Z_PTE v_3).(meta_PA)).(meta_granule_offset)))
-                  (st_1.[share].[globals].[g_granules] :<
-                    ((((st_1.(share)).(globals)).(g_granules)) #
-                      ((((test_Z_PTE v_3).(meta_PA)).(meta_granule_offset)) / (16)) ==
-                      ((((((st_1.(share)).(globals)).(g_granules)) @ ((((test_Z_PTE v_3).(meta_PA)).(meta_granule_offset)) / (16))).[e_ref] :<
-                        ((((((st_1.(share)).(globals)).(g_granules)) @ ((((test_Z_PTE v_3).(meta_PA)).(meta_granule_offset)) / (16))).(e_ref)).[e_u_anon_3_0] :<
-                          ((g_mapped_addr_set_para
-                            ((((((st_1.(share)).(globals)).(g_granules)) @ ((((test_Z_PTE v_3).(meta_PA)).(meta_granule_offset)) / (16))).(e_ref)).(e_u_anon_3_0))
-                            v_1) +
-                            (1)))).[e_state_s_granule] :<
-                        6)))));
-            rely ((((ret_rtt.(e_2)).(pbase)) =s ("granules")));
-            rely ((((((ret_rtt.(e_2)).(poffset)) + (8)) mod (16)) = (8)));
-            when st_19 == (
-                (granule_unlock_spec
-                  (ret_rtt.(e_2))
-                  ((st_6.[share].[globals].[g_granules] :<
-                    ((((st_6.(share)).(globals)).(g_granules)) #
-                      ((((ret_rtt.(e_2)).(poffset)) + (8)) / (16)) ==
-                      (((((st_6.(share)).(globals)).(g_granules)) @ ((((ret_rtt.(e_2)).(poffset)) + (8)) / (16))).[e_ref] :<
-                        ((((((st_6.(share)).(globals)).(g_granules)) @ ((((ret_rtt.(e_2)).(poffset)) + (8)) / (16))).(e_ref)).[e_u_anon_3_0] :<
-                          (((((((st_6.(share)).(globals)).(g_granules)) @ ((((ret_rtt.(e_2)).(poffset)) + (8)) / (16))).(e_ref)).(e_u_anon_3_0)) + (1)))))).[share].[granule_data] :<
-                    (((st_6.(share)).(granule_data)) #
-                      ((((ret_rtt.(e_2)).(poffset)) + ((8 * ((ret_rtt.(e_3)))))) / (4096)) ==
-                      ((((st_6.(share)).(granule_data)) @ ((((ret_rtt.(e_2)).(poffset)) + ((8 * ((ret_rtt.(e_3)))))) / (4096))).[g_norm] :<
-                        (((((st_6.(share)).(granule_data)) @ ((((ret_rtt.(e_2)).(poffset)) + ((8 * ((ret_rtt.(e_3)))))) / (4096))).(g_norm)) #
-                          ((((ret_rtt.(e_2)).(poffset)) + ((8 * ((ret_rtt.(e_3)))))) mod (4096)) ==
-                          (test_PTE_Z (test_Z_PTE v_3))))))));
-            (Some (0, st_19)))
-          else (
-            when st_2 == ((spinlock_release_spec (mkPtr "granules" (((test_Z_PTE v_3).(meta_PA)).(meta_granule_offset))) st_1));
-            when st_5 == ((spinlock_acquire_spec (mkPtr "granules" (((test_Z_PTE v_3).(meta_PA)).(meta_granule_offset))) st_2));
-            if (((((((st_5.(share)).(globals)).(g_granules)) @ ((((test_Z_PTE v_3).(meta_PA)).(meta_granule_offset)) / (16))).(e_state_s_granule)) - (6)) =? (0))
-            then (
-              rely (((((((test_Z_PTE v_3).(meta_PA)).(meta_granule_offset)) mod (16)) = (0)) /\ (((((test_Z_PTE v_3).(meta_PA)).(meta_granule_offset)) >= (0)))));
-              rely (((((((test_Z_PTE v_3).(meta_PA)).(meta_granule_offset)) + (8)) mod (16)) = (8)));
-              when st_6 == (
-                  (granule_unlock_spec
-                    (mkPtr "granules" (((test_Z_PTE v_3).(meta_PA)).(meta_granule_offset)))
-                    (st_5.[share].[globals].[g_granules] :<
-                      ((((st_5.(share)).(globals)).(g_granules)) #
-                        ((((test_Z_PTE v_3).(meta_PA)).(meta_granule_offset)) / (16)) ==
-                        (((((st_5.(share)).(globals)).(g_granules)) @ ((((test_Z_PTE v_3).(meta_PA)).(meta_granule_offset)) / (16))).[e_ref] :<
-                          ((((((st_5.(share)).(globals)).(g_granules)) @ ((((test_Z_PTE v_3).(meta_PA)).(meta_granule_offset)) / (16))).(e_ref)).[e_u_anon_3_0] :<
-                            (((((((st_5.(share)).(globals)).(g_granules)) @ ((((test_Z_PTE v_3).(meta_PA)).(meta_granule_offset)) / (16))).(e_ref)).(e_u_anon_3_0)) + (1))))))));
-              rely ((true = (true)));
-              rely ((((ret_rtt.(e_2)).(pbase)) =s ("granules")));
-              rely ((((((ret_rtt.(e_2)).(poffset)) + (8)) mod (16)) = (8)));
-              when st_19 == (
-                  (granule_unlock_spec
-                    (ret_rtt.(e_2))
-                    ((st_6.[share].[globals].[g_granules] :<
-                      ((((st_6.(share)).(globals)).(g_granules)) #
-                        ((((ret_rtt.(e_2)).(poffset)) + (8)) / (16)) ==
-                        (((((st_6.(share)).(globals)).(g_granules)) @ ((((ret_rtt.(e_2)).(poffset)) + (8)) / (16))).[e_ref] :<
-                          ((((((st_6.(share)).(globals)).(g_granules)) @ ((((ret_rtt.(e_2)).(poffset)) + (8)) / (16))).(e_ref)).[e_u_anon_3_0] :<
-                            (((((((st_6.(share)).(globals)).(g_granules)) @ ((((ret_rtt.(e_2)).(poffset)) + (8)) / (16))).(e_ref)).(e_u_anon_3_0)) + (1)))))).[share].[granule_data] :<
-                      (((st_6.(share)).(granule_data)) #
-                        ((((ret_rtt.(e_2)).(poffset)) + ((8 * ((ret_rtt.(e_3)))))) / (4096)) ==
-                        ((((st_6.(share)).(granule_data)) @ ((((ret_rtt.(e_2)).(poffset)) + ((8 * ((ret_rtt.(e_3)))))) / (4096))).[g_norm] :<
-                          (((((st_6.(share)).(granule_data)) @ ((((ret_rtt.(e_2)).(poffset)) + ((8 * ((ret_rtt.(e_3)))))) / (4096))).(g_norm)) #
-                            ((((ret_rtt.(e_2)).(poffset)) + ((8 * ((ret_rtt.(e_3)))))) mod (4096)) ==
-                            (test_PTE_Z (test_Z_PTE v_3))))))));
-              (Some (0, st_19)))
-            else (
-              when st_6 == ((spinlock_release_spec (mkPtr "granules" (((test_Z_PTE v_3).(meta_PA)).(meta_granule_offset))) st_5));
-              if ((pack_struct_return_code_para (make_return_code_para 1)) =? (0))
-              then (
-                rely ((((ret_rtt.(e_2)).(pbase)) =s ("granules")));
-                rely ((((((ret_rtt.(e_2)).(poffset)) + (8)) mod (16)) = (8)));
-                when st_19 == (
-                    (granule_unlock_spec
-                      (ret_rtt.(e_2))
-                      ((st_6.[share].[globals].[g_granules] :<
-                        ((((st_6.(share)).(globals)).(g_granules)) #
-                          ((((ret_rtt.(e_2)).(poffset)) + (8)) / (16)) ==
-                          (((((st_6.(share)).(globals)).(g_granules)) @ ((((ret_rtt.(e_2)).(poffset)) + (8)) / (16))).[e_ref] :<
-                            ((((((st_6.(share)).(globals)).(g_granules)) @ ((((ret_rtt.(e_2)).(poffset)) + (8)) / (16))).(e_ref)).[e_u_anon_3_0] :<
-                              (((((((st_6.(share)).(globals)).(g_granules)) @ ((((ret_rtt.(e_2)).(poffset)) + (8)) / (16))).(e_ref)).(e_u_anon_3_0)) + (1)))))).[share].[granule_data] :<
-                        (((st_6.(share)).(granule_data)) #
-                          ((((ret_rtt.(e_2)).(poffset)) + ((8 * ((ret_rtt.(e_3)))))) / (4096)) ==
-                          ((((st_6.(share)).(granule_data)) @ ((((ret_rtt.(e_2)).(poffset)) + ((8 * ((ret_rtt.(e_3)))))) / (4096))).[g_norm] :<
-                            (((((st_6.(share)).(granule_data)) @ ((((ret_rtt.(e_2)).(poffset)) + ((8 * ((ret_rtt.(e_3)))))) / (4096))).(g_norm)) #
-                              ((((ret_rtt.(e_2)).(poffset)) + ((8 * ((ret_rtt.(e_3)))))) mod (4096)) ==
-                              (test_PTE_Z (test_Z_PTE v_3))))))));
-                (Some (0, st_19)))
-              else (
-                when st_14 == ((granule_unlock_spec (ret_rtt.(e_2)) st_6));
-                (Some ((pack_struct_return_code_para (make_return_code_para 1)), st_14)))))))
-      else (
-        when st_13 == ((granule_unlock_spec (ret_rtt.(e_2)) st_4));
-        (Some ((pack_struct_return_code_para (make_return_code_para 9)), st_13))))
-    else (
-      if (v_4 =? (1))
-      then (
-        if ((v_2 =? (3)) && ((((abs_tte_read (mkPtr "granule_data" (((ret_rtt.(e_2)).(poffset)) + ((8 * ((ret_rtt.(e_3))))))) st_4).(meta_desc_type)) =? (3))))
-        then (
-          if (uart0_phys_para (abs_tte_read (mkPtr "granule_data" (((ret_rtt.(e_2)).(poffset)) + ((8 * ((ret_rtt.(e_3))))))) st_4))
-          then (
-            rely ((((((ret_rtt.(e_2)).(pbase)) = ("granules")) /\ (((((ret_rtt.(e_2)).(poffset)) mod (16)) = (0)))) /\ ((((ret_rtt.(e_2)).(poffset)) >= (0)))));
-            when st_19 == (
-                (granule_unlock_spec
-                  (ret_rtt.(e_2))
-                  ((st_4.[share].[globals].[g_granules] :<
-                    ((((st_4.(share)).(globals)).(g_granules)) #
-                      (((ret_rtt.(e_2)).(poffset)) / (16)) ==
-                      (((((st_4.(share)).(globals)).(g_granules)) @ (((ret_rtt.(e_2)).(poffset)) / (16))).[e_ref] :<
-                        ((((((st_4.(share)).(globals)).(g_granules)) @ (((ret_rtt.(e_2)).(poffset)) / (16))).(e_ref)).[e_u_anon_3_0] :<
-                          (((((((st_4.(share)).(globals)).(g_granules)) @ (((ret_rtt.(e_2)).(poffset)) / (16))).(e_ref)).(e_u_anon_3_0)) + ((- 1))))))).[share].[granule_data] :<
-                    (((st_4.(share)).(granule_data)) #
-                      ((((ret_rtt.(e_2)).(poffset)) + ((8 * ((ret_rtt.(e_3)))))) / (4096)) ==
-                      ((((st_4.(share)).(granule_data)) @ ((((ret_rtt.(e_2)).(poffset)) + ((8 * ((ret_rtt.(e_3)))))) / (4096))).[g_norm] :<
-                        (((((st_4.(share)).(granule_data)) @ ((((ret_rtt.(e_2)).(poffset)) + ((8 * ((ret_rtt.(e_3)))))) / (4096))).(g_norm)) #
-                          ((((ret_rtt.(e_2)).(poffset)) + ((8 * ((ret_rtt.(e_3)))))) mod (4096)) ==
-                          (test_PTE_Z (mkabs_PTE_t (mkabs_PA_t (- 1)) 0 1))))))));
-            (Some (0, st_19)))
-          else (
-            when st_1 == (
-                (spinlock_acquire_spec
-                  (mkPtr "granules" (((abs_tte_read (mkPtr "granule_data" (((ret_rtt.(e_2)).(poffset)) + ((8 * ((ret_rtt.(e_3))))))) st_4).(meta_PA)).(meta_granule_offset)))
-                  st_4));
-            if (
-              (((((((st_1.(share)).(globals)).(g_granules)) @ ((((abs_tte_read (mkPtr "granule_data" (((ret_rtt.(e_2)).(poffset)) + ((8 * ((ret_rtt.(e_3))))))) st_4).(meta_PA)).(meta_granule_offset)) / (16))).(e_state_s_granule)) -
-                (6)) =?
-                (0)))
-            then (
-              rely (
-                ((((((abs_tte_read (mkPtr "granule_data" (((ret_rtt.(e_2)).(poffset)) + ((8 * ((ret_rtt.(e_3))))))) st_4).(meta_PA)).(meta_granule_offset)) mod (16)) = (0)) /\
-                  (((((abs_tte_read (mkPtr "granule_data" (((ret_rtt.(e_2)).(poffset)) + ((8 * ((ret_rtt.(e_3))))))) st_4).(meta_PA)).(meta_granule_offset)) >= (0)))));
-              if (
-                ((g_refcount_para
-                  (mkPtr "granules" (((abs_tte_read (mkPtr "granule_data" (((ret_rtt.(e_2)).(poffset)) + ((8 * ((ret_rtt.(e_3))))))) st_4).(meta_PA)).(meta_granule_offset)))
-                  (st_1.[share].[globals].[g_granules] :<
-                    ((((st_1.(share)).(globals)).(g_granules)) #
-                      ((((abs_tte_read (mkPtr "granule_data" (((ret_rtt.(e_2)).(poffset)) + ((8 * ((ret_rtt.(e_3))))))) st_4).(meta_PA)).(meta_granule_offset)) / (16)) ==
-                      (((((st_1.(share)).(globals)).(g_granules)) @ ((((abs_tte_read (mkPtr "granule_data" (((ret_rtt.(e_2)).(poffset)) + ((8 * ((ret_rtt.(e_3))))))) st_4).(meta_PA)).(meta_granule_offset)) / (16))).[e_ref] :<
-                        ((((((st_1.(share)).(globals)).(g_granules)) @ ((((abs_tte_read (mkPtr "granule_data" (((ret_rtt.(e_2)).(poffset)) + ((8 * ((ret_rtt.(e_3))))))) st_4).(meta_PA)).(meta_granule_offset)) / (16))).(e_ref)).[e_u_anon_3_0] :<
-                          (((((((st_1.(share)).(globals)).(g_granules)) @ ((((abs_tte_read (mkPtr "granule_data" (((ret_rtt.(e_2)).(poffset)) + ((8 * ((ret_rtt.(e_3))))))) st_4).(meta_PA)).(meta_granule_offset)) / (16))).(e_ref)).(e_u_anon_3_0)) +
-                            ((- 1)))))))) =?
-                  (0)))
-              then (
-                when st_7 == (
-                    (granule_unlock_spec
-                      (mkPtr "granules" (((abs_tte_read (mkPtr "granule_data" (((ret_rtt.(e_2)).(poffset)) + ((8 * ((ret_rtt.(e_3))))))) st_4).(meta_PA)).(meta_granule_offset)))
-                      (st_1.[share].[globals].[g_granules] :<
-                        ((((st_1.(share)).(globals)).(g_granules)) #
-                          ((((abs_tte_read (mkPtr "granule_data" (((ret_rtt.(e_2)).(poffset)) + ((8 * ((ret_rtt.(e_3))))))) st_4).(meta_PA)).(meta_granule_offset)) / (16)) ==
-                          ((((((st_1.(share)).(globals)).(g_granules)) @ ((((abs_tte_read (mkPtr "granule_data" (((ret_rtt.(e_2)).(poffset)) + ((8 * ((ret_rtt.(e_3))))))) st_4).(meta_PA)).(meta_granule_offset)) / (16))).[e_ref] :<
-                            ((((((st_1.(share)).(globals)).(g_granules)) @ ((((abs_tte_read (mkPtr "granule_data" (((ret_rtt.(e_2)).(poffset)) + ((8 * ((ret_rtt.(e_3))))))) st_4).(meta_PA)).(meta_granule_offset)) / (16))).(e_ref)).[e_u_anon_3_0] :<
-                              (g_mapped_addr_set_para
-                                (((((((st_1.(share)).(globals)).(g_granules)) @ ((((abs_tte_read (mkPtr "granule_data" (((ret_rtt.(e_2)).(poffset)) + ((8 * ((ret_rtt.(e_3))))))) st_4).(meta_PA)).(meta_granule_offset)) / (16))).(e_ref)).(e_u_anon_3_0)) +
-                                  ((- 1)))
-                                0))).[e_state_s_granule] :<
-                            0)))));
-                rely ((((((ret_rtt.(e_2)).(pbase)) = ("granules")) /\ (((((ret_rtt.(e_2)).(poffset)) mod (16)) = (0)))) /\ ((((ret_rtt.(e_2)).(poffset)) >= (0)))));
-                when st_20 == (
-                    (granule_unlock_spec
-                      (ret_rtt.(e_2))
-                      ((st_7.[share].[globals].[g_granules] :<
-                        ((((st_7.(share)).(globals)).(g_granules)) #
-                          (((ret_rtt.(e_2)).(poffset)) / (16)) ==
-                          (((((st_7.(share)).(globals)).(g_granules)) @ (((ret_rtt.(e_2)).(poffset)) / (16))).[e_ref] :<
-                            ((((((st_7.(share)).(globals)).(g_granules)) @ (((ret_rtt.(e_2)).(poffset)) / (16))).(e_ref)).[e_u_anon_3_0] :<
-                              (((((((st_7.(share)).(globals)).(g_granules)) @ (((ret_rtt.(e_2)).(poffset)) / (16))).(e_ref)).(e_u_anon_3_0)) + ((- 1))))))).[share].[granule_data] :<
-                        (((st_7.(share)).(granule_data)) #
-                          ((((ret_rtt.(e_2)).(poffset)) + ((8 * ((ret_rtt.(e_3)))))) / (4096)) ==
-                          ((((st_7.(share)).(granule_data)) @ ((((ret_rtt.(e_2)).(poffset)) + ((8 * ((ret_rtt.(e_3)))))) / (4096))).[g_norm] :<
-                            (((((st_7.(share)).(granule_data)) @ ((((ret_rtt.(e_2)).(poffset)) + ((8 * ((ret_rtt.(e_3)))))) / (4096))).(g_norm)) #
-                              ((((ret_rtt.(e_2)).(poffset)) + ((8 * ((ret_rtt.(e_3)))))) mod (4096)) ==
-                              (test_PTE_Z (mkabs_PTE_t (mkabs_PA_t (- 1)) 0 1))))))));
-                (Some (0, st_20)))
-              else (
-                when st_5 == (
-                    (granule_unlock_spec
-                      (mkPtr "granules" (((abs_tte_read (mkPtr "granule_data" (((ret_rtt.(e_2)).(poffset)) + ((8 * ((ret_rtt.(e_3))))))) st_4).(meta_PA)).(meta_granule_offset)))
-                      (st_1.[share].[globals].[g_granules] :<
-                        ((((st_1.(share)).(globals)).(g_granules)) #
-                          ((((abs_tte_read (mkPtr "granule_data" (((ret_rtt.(e_2)).(poffset)) + ((8 * ((ret_rtt.(e_3))))))) st_4).(meta_PA)).(meta_granule_offset)) / (16)) ==
-                          (((((st_1.(share)).(globals)).(g_granules)) @ ((((abs_tte_read (mkPtr "granule_data" (((ret_rtt.(e_2)).(poffset)) + ((8 * ((ret_rtt.(e_3))))))) st_4).(meta_PA)).(meta_granule_offset)) / (16))).[e_ref] :<
-                            ((((((st_1.(share)).(globals)).(g_granules)) @ ((((abs_tte_read (mkPtr "granule_data" (((ret_rtt.(e_2)).(poffset)) + ((8 * ((ret_rtt.(e_3))))))) st_4).(meta_PA)).(meta_granule_offset)) / (16))).(e_ref)).[e_u_anon_3_0] :<
-                              (g_mapped_addr_set_para
-                                (((((((st_1.(share)).(globals)).(g_granules)) @ ((((abs_tte_read (mkPtr "granule_data" (((ret_rtt.(e_2)).(poffset)) + ((8 * ((ret_rtt.(e_3))))))) st_4).(meta_PA)).(meta_granule_offset)) / (16))).(e_ref)).(e_u_anon_3_0)) +
-                                  ((- 1)))
-                                0)))))));
-                rely ((((((ret_rtt.(e_2)).(pbase)) = ("granules")) /\ (((((ret_rtt.(e_2)).(poffset)) mod (16)) = (0)))) /\ ((((ret_rtt.(e_2)).(poffset)) >= (0)))));
-                when st_20 == (
-                    (granule_unlock_spec
-                      (ret_rtt.(e_2))
-                      ((st_5.[share].[globals].[g_granules] :<
-                        ((((st_5.(share)).(globals)).(g_granules)) #
-                          (((ret_rtt.(e_2)).(poffset)) / (16)) ==
-                          (((((st_5.(share)).(globals)).(g_granules)) @ (((ret_rtt.(e_2)).(poffset)) / (16))).[e_ref] :<
-                            ((((((st_5.(share)).(globals)).(g_granules)) @ (((ret_rtt.(e_2)).(poffset)) / (16))).(e_ref)).[e_u_anon_3_0] :<
-                              (((((((st_5.(share)).(globals)).(g_granules)) @ (((ret_rtt.(e_2)).(poffset)) / (16))).(e_ref)).(e_u_anon_3_0)) + ((- 1))))))).[share].[granule_data] :<
-                        (((st_5.(share)).(granule_data)) #
-                          ((((ret_rtt.(e_2)).(poffset)) + ((8 * ((ret_rtt.(e_3)))))) / (4096)) ==
-                          ((((st_5.(share)).(granule_data)) @ ((((ret_rtt.(e_2)).(poffset)) + ((8 * ((ret_rtt.(e_3)))))) / (4096))).[g_norm] :<
-                            (((((st_5.(share)).(granule_data)) @ ((((ret_rtt.(e_2)).(poffset)) + ((8 * ((ret_rtt.(e_3)))))) / (4096))).(g_norm)) #
-                              ((((ret_rtt.(e_2)).(poffset)) + ((8 * ((ret_rtt.(e_3)))))) mod (4096)) ==
-                              (test_PTE_Z (mkabs_PTE_t (mkabs_PA_t (- 1)) 0 1))))))));
-                (Some (0, st_20))))
-            else (
-              when st_2 == (
-                  (spinlock_release_spec
-                    (mkPtr "granules" (((abs_tte_read (mkPtr "granule_data" (((ret_rtt.(e_2)).(poffset)) + ((8 * ((ret_rtt.(e_3))))))) st_4).(meta_PA)).(meta_granule_offset)))
-                    st_1));
-              if ((pack_struct_return_code_para (make_return_code_para 1)) =? (0))
-              then (
-                rely ((((((ret_rtt.(e_2)).(pbase)) = ("granules")) /\ (((((ret_rtt.(e_2)).(poffset)) mod (16)) = (0)))) /\ ((((ret_rtt.(e_2)).(poffset)) >= (0)))));
-                when st_20 == (
-                    (granule_unlock_spec
-                      (ret_rtt.(e_2))
-                      ((st_2.[share].[globals].[g_granules] :<
-                        ((((st_2.(share)).(globals)).(g_granules)) #
-                          (((ret_rtt.(e_2)).(poffset)) / (16)) ==
-                          (((((st_2.(share)).(globals)).(g_granules)) @ (((ret_rtt.(e_2)).(poffset)) / (16))).[e_ref] :<
-                            ((((((st_2.(share)).(globals)).(g_granules)) @ (((ret_rtt.(e_2)).(poffset)) / (16))).(e_ref)).[e_u_anon_3_0] :<
-                              (((((((st_2.(share)).(globals)).(g_granules)) @ (((ret_rtt.(e_2)).(poffset)) / (16))).(e_ref)).(e_u_anon_3_0)) + ((- 1))))))).[share].[granule_data] :<
-                        (((st_2.(share)).(granule_data)) #
-                          ((((ret_rtt.(e_2)).(poffset)) + ((8 * ((ret_rtt.(e_3)))))) / (4096)) ==
-                          ((((st_2.(share)).(granule_data)) @ ((((ret_rtt.(e_2)).(poffset)) + ((8 * ((ret_rtt.(e_3)))))) / (4096))).[g_norm] :<
-                            (((((st_2.(share)).(granule_data)) @ ((((ret_rtt.(e_2)).(poffset)) + ((8 * ((ret_rtt.(e_3)))))) / (4096))).(g_norm)) #
-                              ((((ret_rtt.(e_2)).(poffset)) + ((8 * ((ret_rtt.(e_3)))))) mod (4096)) ==
-                              (test_PTE_Z (mkabs_PTE_t (mkabs_PA_t (- 1)) 0 1))))))));
-                (Some (0, st_20)))
-              else (
-                when st_14 == ((granule_unlock_spec (ret_rtt.(e_2)) st_2));
-                (Some ((pack_struct_return_code_para (make_return_code_para 1)), st_14))))))
-        else (
-          if ((v_2 <>? (3)) && ((((abs_tte_read (mkPtr "granule_data" (((ret_rtt.(e_2)).(poffset)) + ((8 * ((ret_rtt.(e_3))))))) st_4).(meta_desc_type)) =? (1))))
-          then (
-            if (uart0_phys_para (abs_tte_read (mkPtr "granule_data" (((ret_rtt.(e_2)).(poffset)) + ((8 * ((ret_rtt.(e_3))))))) st_4))
-            then (
-              rely ((((((ret_rtt.(e_2)).(pbase)) = ("granules")) /\ (((((ret_rtt.(e_2)).(poffset)) mod (16)) = (0)))) /\ ((((ret_rtt.(e_2)).(poffset)) >= (0)))));
-              when st_19 == (
-                  (granule_unlock_spec
-                    (ret_rtt.(e_2))
-                    ((st_4.[share].[globals].[g_granules] :<
-                      ((((st_4.(share)).(globals)).(g_granules)) #
-                        (((ret_rtt.(e_2)).(poffset)) / (16)) ==
-                        (((((st_4.(share)).(globals)).(g_granules)) @ (((ret_rtt.(e_2)).(poffset)) / (16))).[e_ref] :<
-                          ((((((st_4.(share)).(globals)).(g_granules)) @ (((ret_rtt.(e_2)).(poffset)) / (16))).(e_ref)).[e_u_anon_3_0] :<
-                            (((((((st_4.(share)).(globals)).(g_granules)) @ (((ret_rtt.(e_2)).(poffset)) / (16))).(e_ref)).(e_u_anon_3_0)) + ((- 1))))))).[share].[granule_data] :<
-                      (((st_4.(share)).(granule_data)) #
-                        ((((ret_rtt.(e_2)).(poffset)) + ((8 * ((ret_rtt.(e_3)))))) / (4096)) ==
-                        ((((st_4.(share)).(granule_data)) @ ((((ret_rtt.(e_2)).(poffset)) + ((8 * ((ret_rtt.(e_3)))))) / (4096))).[g_norm] :<
-                          (((((st_4.(share)).(granule_data)) @ ((((ret_rtt.(e_2)).(poffset)) + ((8 * ((ret_rtt.(e_3)))))) / (4096))).(g_norm)) #
-                            ((((ret_rtt.(e_2)).(poffset)) + ((8 * ((ret_rtt.(e_3)))))) mod (4096)) ==
-                            (test_PTE_Z (mkabs_PTE_t (mkabs_PA_t (- 1)) 0 1))))))));
-              (Some (0, st_19)))
-            else (
-              when st_1 == (
-                  (spinlock_acquire_spec
-                    (mkPtr "granules" (((abs_tte_read (mkPtr "granule_data" (((ret_rtt.(e_2)).(poffset)) + ((8 * ((ret_rtt.(e_3))))))) st_4).(meta_PA)).(meta_granule_offset)))
-                    st_4));
-              if (
-                (((((((st_1.(share)).(globals)).(g_granules)) @ ((((abs_tte_read (mkPtr "granule_data" (((ret_rtt.(e_2)).(poffset)) + ((8 * ((ret_rtt.(e_3))))))) st_4).(meta_PA)).(meta_granule_offset)) / (16))).(e_state_s_granule)) -
-                  (6)) =?
-                  (0)))
-              then (
-                rely (
-                  ((((((abs_tte_read (mkPtr "granule_data" (((ret_rtt.(e_2)).(poffset)) + ((8 * ((ret_rtt.(e_3))))))) st_4).(meta_PA)).(meta_granule_offset)) mod (16)) = (0)) /\
-                    (((((abs_tte_read (mkPtr "granule_data" (((ret_rtt.(e_2)).(poffset)) + ((8 * ((ret_rtt.(e_3))))))) st_4).(meta_PA)).(meta_granule_offset)) >= (0)))));
-                if (
-                  ((g_refcount_para
-                    (mkPtr "granules" (((abs_tte_read (mkPtr "granule_data" (((ret_rtt.(e_2)).(poffset)) + ((8 * ((ret_rtt.(e_3))))))) st_4).(meta_PA)).(meta_granule_offset)))
-                    (st_1.[share].[globals].[g_granules] :<
-                      ((((st_1.(share)).(globals)).(g_granules)) #
-                        ((((abs_tte_read (mkPtr "granule_data" (((ret_rtt.(e_2)).(poffset)) + ((8 * ((ret_rtt.(e_3))))))) st_4).(meta_PA)).(meta_granule_offset)) / (16)) ==
-                        (((((st_1.(share)).(globals)).(g_granules)) @ ((((abs_tte_read (mkPtr "granule_data" (((ret_rtt.(e_2)).(poffset)) + ((8 * ((ret_rtt.(e_3))))))) st_4).(meta_PA)).(meta_granule_offset)) / (16))).[e_ref] :<
-                          ((((((st_1.(share)).(globals)).(g_granules)) @ ((((abs_tte_read (mkPtr "granule_data" (((ret_rtt.(e_2)).(poffset)) + ((8 * ((ret_rtt.(e_3))))))) st_4).(meta_PA)).(meta_granule_offset)) / (16))).(e_ref)).[e_u_anon_3_0] :<
-                            (((((((st_1.(share)).(globals)).(g_granules)) @ ((((abs_tte_read (mkPtr "granule_data" (((ret_rtt.(e_2)).(poffset)) + ((8 * ((ret_rtt.(e_3))))))) st_4).(meta_PA)).(meta_granule_offset)) / (16))).(e_ref)).(e_u_anon_3_0)) +
-                              ((- 1)))))))) =?
-                    (0)))
-                then (
-                  when st_7 == (
-                      (granule_unlock_spec
-                        (mkPtr "granules" (((abs_tte_read (mkPtr "granule_data" (((ret_rtt.(e_2)).(poffset)) + ((8 * ((ret_rtt.(e_3))))))) st_4).(meta_PA)).(meta_granule_offset)))
-                        (st_1.[share].[globals].[g_granules] :<
-                          ((((st_1.(share)).(globals)).(g_granules)) #
-                            ((((abs_tte_read (mkPtr "granule_data" (((ret_rtt.(e_2)).(poffset)) + ((8 * ((ret_rtt.(e_3))))))) st_4).(meta_PA)).(meta_granule_offset)) / (16)) ==
-                            ((((((st_1.(share)).(globals)).(g_granules)) @ ((((abs_tte_read (mkPtr "granule_data" (((ret_rtt.(e_2)).(poffset)) + ((8 * ((ret_rtt.(e_3))))))) st_4).(meta_PA)).(meta_granule_offset)) / (16))).[e_ref] :<
-                              ((((((st_1.(share)).(globals)).(g_granules)) @ ((((abs_tte_read (mkPtr "granule_data" (((ret_rtt.(e_2)).(poffset)) + ((8 * ((ret_rtt.(e_3))))))) st_4).(meta_PA)).(meta_granule_offset)) / (16))).(e_ref)).[e_u_anon_3_0] :<
-                                (g_mapped_addr_set_para
-                                  (((((((st_1.(share)).(globals)).(g_granules)) @ ((((abs_tte_read (mkPtr "granule_data" (((ret_rtt.(e_2)).(poffset)) + ((8 * ((ret_rtt.(e_3))))))) st_4).(meta_PA)).(meta_granule_offset)) / (16))).(e_ref)).(e_u_anon_3_0)) +
-                                    ((- 1)))
-                                  0))).[e_state_s_granule] :<
-                              0)))));
-                  rely ((true = (true)));
-                  rely ((((((ret_rtt.(e_2)).(pbase)) = ("granules")) /\ (((((ret_rtt.(e_2)).(poffset)) mod (16)) = (0)))) /\ ((((ret_rtt.(e_2)).(poffset)) >= (0)))));
-                  when st_20 == (
-                      (granule_unlock_spec
-                        (ret_rtt.(e_2))
-                        ((st_7.[share].[globals].[g_granules] :<
-                          ((((st_7.(share)).(globals)).(g_granules)) #
-                            (((ret_rtt.(e_2)).(poffset)) / (16)) ==
-                            (((((st_7.(share)).(globals)).(g_granules)) @ (((ret_rtt.(e_2)).(poffset)) / (16))).[e_ref] :<
-                              ((((((st_7.(share)).(globals)).(g_granules)) @ (((ret_rtt.(e_2)).(poffset)) / (16))).(e_ref)).[e_u_anon_3_0] :<
-                                (((((((st_7.(share)).(globals)).(g_granules)) @ (((ret_rtt.(e_2)).(poffset)) / (16))).(e_ref)).(e_u_anon_3_0)) + ((- 1))))))).[share].[granule_data] :<
-                          (((st_7.(share)).(granule_data)) #
-                            ((((ret_rtt.(e_2)).(poffset)) + ((8 * ((ret_rtt.(e_3)))))) / (4096)) ==
-                            ((((st_7.(share)).(granule_data)) @ ((((ret_rtt.(e_2)).(poffset)) + ((8 * ((ret_rtt.(e_3)))))) / (4096))).[g_norm] :<
-                              (((((st_7.(share)).(granule_data)) @ ((((ret_rtt.(e_2)).(poffset)) + ((8 * ((ret_rtt.(e_3)))))) / (4096))).(g_norm)) #
-                                ((((ret_rtt.(e_2)).(poffset)) + ((8 * ((ret_rtt.(e_3)))))) mod (4096)) ==
-                                (test_PTE_Z (mkabs_PTE_t (mkabs_PA_t (- 1)) 0 1))))))));
-                  (Some (0, st_20)))
-                else (
-                  when st_5 == (
-                      (granule_unlock_spec
-                        (mkPtr "granules" (((abs_tte_read (mkPtr "granule_data" (((ret_rtt.(e_2)).(poffset)) + ((8 * ((ret_rtt.(e_3))))))) st_4).(meta_PA)).(meta_granule_offset)))
-                        (st_1.[share].[globals].[g_granules] :<
-                          ((((st_1.(share)).(globals)).(g_granules)) #
-                            ((((abs_tte_read (mkPtr "granule_data" (((ret_rtt.(e_2)).(poffset)) + ((8 * ((ret_rtt.(e_3))))))) st_4).(meta_PA)).(meta_granule_offset)) / (16)) ==
-                            (((((st_1.(share)).(globals)).(g_granules)) @ ((((abs_tte_read (mkPtr "granule_data" (((ret_rtt.(e_2)).(poffset)) + ((8 * ((ret_rtt.(e_3))))))) st_4).(meta_PA)).(meta_granule_offset)) / (16))).[e_ref] :<
-                              ((((((st_1.(share)).(globals)).(g_granules)) @ ((((abs_tte_read (mkPtr "granule_data" (((ret_rtt.(e_2)).(poffset)) + ((8 * ((ret_rtt.(e_3))))))) st_4).(meta_PA)).(meta_granule_offset)) / (16))).(e_ref)).[e_u_anon_3_0] :<
-                                (g_mapped_addr_set_para
-                                  (((((((st_1.(share)).(globals)).(g_granules)) @ ((((abs_tte_read (mkPtr "granule_data" (((ret_rtt.(e_2)).(poffset)) + ((8 * ((ret_rtt.(e_3))))))) st_4).(meta_PA)).(meta_granule_offset)) / (16))).(e_ref)).(e_u_anon_3_0)) +
-                                    ((- 1)))
-                                  0)))))));
-                  rely ((true = (true)));
-                  rely ((((((ret_rtt.(e_2)).(pbase)) = ("granules")) /\ (((((ret_rtt.(e_2)).(poffset)) mod (16)) = (0)))) /\ ((((ret_rtt.(e_2)).(poffset)) >= (0)))));
-                  when st_20 == (
-                      (granule_unlock_spec
-                        (ret_rtt.(e_2))
-                        ((st_5.[share].[globals].[g_granules] :<
-                          ((((st_5.(share)).(globals)).(g_granules)) #
-                            (((ret_rtt.(e_2)).(poffset)) / (16)) ==
-                            (((((st_5.(share)).(globals)).(g_granules)) @ (((ret_rtt.(e_2)).(poffset)) / (16))).[e_ref] :<
-                              ((((((st_5.(share)).(globals)).(g_granules)) @ (((ret_rtt.(e_2)).(poffset)) / (16))).(e_ref)).[e_u_anon_3_0] :<
-                                (((((((st_5.(share)).(globals)).(g_granules)) @ (((ret_rtt.(e_2)).(poffset)) / (16))).(e_ref)).(e_u_anon_3_0)) + ((- 1))))))).[share].[granule_data] :<
-                          (((st_5.(share)).(granule_data)) #
-                            ((((ret_rtt.(e_2)).(poffset)) + ((8 * ((ret_rtt.(e_3)))))) / (4096)) ==
-                            ((((st_5.(share)).(granule_data)) @ ((((ret_rtt.(e_2)).(poffset)) + ((8 * ((ret_rtt.(e_3)))))) / (4096))).[g_norm] :<
-                              (((((st_5.(share)).(granule_data)) @ ((((ret_rtt.(e_2)).(poffset)) + ((8 * ((ret_rtt.(e_3)))))) / (4096))).(g_norm)) #
-                                ((((ret_rtt.(e_2)).(poffset)) + ((8 * ((ret_rtt.(e_3)))))) mod (4096)) ==
-                                (test_PTE_Z (mkabs_PTE_t (mkabs_PA_t (- 1)) 0 1))))))));
-                  (Some (0, st_20))))
-              else (
-                when st_2 == (
-                    (spinlock_release_spec
-                      (mkPtr "granules" (((abs_tte_read (mkPtr "granule_data" (((ret_rtt.(e_2)).(poffset)) + ((8 * ((ret_rtt.(e_3))))))) st_4).(meta_PA)).(meta_granule_offset)))
-                      st_1));
-                if ((pack_struct_return_code_para (make_return_code_para 1)) =? (0))
-                then (
-                  rely ((((((ret_rtt.(e_2)).(pbase)) = ("granules")) /\ (((((ret_rtt.(e_2)).(poffset)) mod (16)) = (0)))) /\ ((((ret_rtt.(e_2)).(poffset)) >= (0)))));
-                  when st_20 == (
-                      (granule_unlock_spec
-                        (ret_rtt.(e_2))
-                        ((st_2.[share].[globals].[g_granules] :<
-                          ((((st_2.(share)).(globals)).(g_granules)) #
-                            (((ret_rtt.(e_2)).(poffset)) / (16)) ==
-                            (((((st_2.(share)).(globals)).(g_granules)) @ (((ret_rtt.(e_2)).(poffset)) / (16))).[e_ref] :<
-                              ((((((st_2.(share)).(globals)).(g_granules)) @ (((ret_rtt.(e_2)).(poffset)) / (16))).(e_ref)).[e_u_anon_3_0] :<
-                                (((((((st_2.(share)).(globals)).(g_granules)) @ (((ret_rtt.(e_2)).(poffset)) / (16))).(e_ref)).(e_u_anon_3_0)) + ((- 1))))))).[share].[granule_data] :<
-                          (((st_2.(share)).(granule_data)) #
-                            ((((ret_rtt.(e_2)).(poffset)) + ((8 * ((ret_rtt.(e_3)))))) / (4096)) ==
-                            ((((st_2.(share)).(granule_data)) @ ((((ret_rtt.(e_2)).(poffset)) + ((8 * ((ret_rtt.(e_3)))))) / (4096))).[g_norm] :<
-                              (((((st_2.(share)).(granule_data)) @ ((((ret_rtt.(e_2)).(poffset)) + ((8 * ((ret_rtt.(e_3)))))) / (4096))).(g_norm)) #
-                                ((((ret_rtt.(e_2)).(poffset)) + ((8 * ((ret_rtt.(e_3)))))) mod (4096)) ==
-                                (test_PTE_Z (mkabs_PTE_t (mkabs_PA_t (- 1)) 0 1))))))));
-                  (Some (0, st_20)))
-                else (
-                  when st_14 == ((granule_unlock_spec (ret_rtt.(e_2)) st_2));
-                  (Some ((pack_struct_return_code_para (make_return_code_para 1)), st_14))))))
-          else (
-            when st_13 == ((granule_unlock_spec (ret_rtt.(e_2)) st_4));
-            (Some ((pack_struct_return_code_para (make_return_code_para 9)), st_13)))))
-      else (
-        when st_12 == ((granule_unlock_spec (ret_rtt.(e_2)) st_4));
-        (Some (0, st_12)))))
+Definition update_ripas_spec (v_0: Ptr) (v_1: Z) (v_2: Z) (st: RData) : (option (bool * RData)) :=
+  if ((v_1 <? (3)) && ((((test_Ptr_PTE v_0).(meta_desc_type)) =? (3))))
+  then (Some (false, st))
   else (
-    when st_8 == ((granule_unlock_spec (ret_rtt.(e_2)) st_4));
-    (Some ((pack_struct_return_code_para (make_return_code_para 8)), st_8))).
+    if ((v_1 =? (3)) && ((((test_Ptr_PTE v_0).(meta_desc_type)) =? (3))))
+    then (Some (true, st))
+    else (
+      if ((v_1 <>? (3)) && ((((test_Ptr_PTE v_0).(meta_desc_type)) =? (1))))
+      then (Some (true, st))
+      else (
+        if (((((test_Ptr_PTE v_0).(meta_desc_type)) =? (0)) && ((((test_Ptr_PTE v_0).(meta_ripas)) =? (0)))) && ((((test_Ptr_PTE v_0).(meta_mem_attr)) =? (0))))
+        then (Some (true, st))
+        else (
+          if (((((test_Ptr_PTE v_0).(meta_desc_type)) =? (0)) && ((((test_Ptr_PTE v_0).(meta_ripas)) =? (0)))) && ((((test_Ptr_PTE v_0).(meta_mem_attr)) =? (1))))
+          then (Some (true, st))
+          else (Some (false, st)))))).
 
