container/coq/pointer/Layer5/Spec.v
@@ -22,7 +22,7 @@ Section Layer5_Spec.
   Context `{int_ptr: IntPtrCast}.
 
   Definition s2tte_create_unassigned_spec_abs (v_0: Z) (st: RData) : (option (abs_PTE_t * RData)) :=
-    (Some ((mkabs_PTE_t (mkabs_PA_t (- 1)) 0 v_0), st)).
+    (Some ((mkabs_PTE_t (mkabs_PA_t (- 1)) 0 v_0 0), st)).
 
   Definition llvm_memset_p0i8_i64_spec (v_0: Ptr) (arg1: Z) (arg2: Z) (arg3: bool) (st: RData) : (option RData) :=
     when st_0 == ((llvm_memset_p0i8_i64_spec_state_oracle v_0 arg1 arg2 arg3 st));
@@ -66,6 +66,9 @@ Section Layer5_Spec.
     when st_2 == ((store_RData_granules 64 loc (v + (val)) st_1));
     (Some st_2).
 
+  Definition s2tte_is_table_spec (v_0: Z) (v_1: Z) (st: RData) : (option (bool * RData)) :=
+    (Some (((v_1 <? (3)) && (((v_0 & (3)) =? (3)))), st)).
+
   Definition granule_unlock_spec (v_0: Ptr) (st: RData) : (option RData) :=
     when st_0 == ((spinlock_release_spec (mkPtr (v_0.(pbase)) (v_0.(poffset))) st));
     (Some st_0).
@@ -93,33 +96,8 @@ Section Layer5_Spec.
   Definition make_return_code_spec (v_0: Z) (v_1: Z) (st: RData) : (option (Z * RData)) :=
     (Some ((make_return_code_para v_0), st)).
 
-  Definition atomic_granule_get_spec (v_0: Ptr) (st: RData) : (option RData) :=
-    rely (((v_0.(pbase)) =s ("granules")));
-    rely (((((v_0.(poffset)) + (8)) mod (16)) = (8)));
-    (Some (st.[share].[globals].[g_granules] :<
-      ((((st.(share)).(globals)).(g_granules)) #
-        (((v_0.(poffset)) + (8)) / (16)) ==
-        (((((st.(share)).(globals)).(g_granules)) @ (((v_0.(poffset)) + (8)) / (16))).[e_ref] :<
-          ((((((st.(share)).(globals)).(g_granules)) @ (((v_0.(poffset)) + (8)) / (16))).(e_ref)).[e_u_anon_3_0] :<
-            (((((((st.(share)).(globals)).(g_granules)) @ (((v_0.(poffset)) + (8)) / (16))).(e_ref)).(e_u_anon_3_0)) + (1))))))).
-
-  Definition atomic_granule_put_spec (v_0: Ptr) (st: RData) : (option RData) :=
-    rely (((v_0.(pbase)) =s ("granules")));
-    rely (((((v_0.(poffset)) + (8)) mod (16)) = (8)));
-    (Some (st.[share].[globals].[g_granules] :<
-      ((((st.(share)).(globals)).(g_granules)) #
-        (((v_0.(poffset)) + (8)) / (16)) ==
-        (((((st.(share)).(globals)).(g_granules)) @ (((v_0.(poffset)) + (8)) / (16))).[e_ref] :<
-          ((((((st.(share)).(globals)).(g_granules)) @ (((v_0.(poffset)) + (8)) / (16))).(e_ref)).[e_u_anon_3_0] :<
-            (((((((st.(share)).(globals)).(g_granules)) @ (((v_0.(poffset)) + (8)) / (16))).(e_ref)).(e_u_anon_3_0)) + ((- 1)))))))).
-
   Definition find_lock_granule_spec (v_0: abs_PA_t) (v_1: Z) (st: RData) : (option (Ptr * RData)) :=
     None.
-
-  Definition s2tte_create_unassigned_spec (v_0: Z) (st: RData) : (option (Z * RData)) :=
-    if (v_0 =? (0))
-    then (Some (0, st))
-    else (Some (64, st)).
 
 End Layer5_Spec.
 
@@ -132,12 +110,10 @@ End Layer5_Spec.
 #[global] Hint Unfold __find_lock_next_level_spec_low_abs: spec.
 #[global] Hint Unfold find_lock_granule_spec_abs: spec.
 #[global] Hint Unfold atomic_add_64: spec.
+#[global] Hint Unfold s2tte_is_table_spec: spec.
 Opaque granule_unlock_spec.
 #[global] Hint Unfold s2_sl_addr_to_idx_spec: spec.
 #[global] Hint Unfold __find_lock_next_level_spec: spec.
 #[global] Hint Unfold pack_struct_return_code_spec: spec.
 #[global] Hint Unfold make_return_code_spec: spec.
-#[global] Hint Unfold atomic_granule_get_spec: spec.
-#[global] Hint Unfold atomic_granule_put_spec: spec.
 #[global] Hint Unfold find_lock_granule_spec: spec.
-#[global] Hint Unfold s2tte_create_unassigned_spec: spec.
