container/coq/pointer/Layer6/s2tte_pa/LowSpec.v
@@ -13,9 +13,14 @@ Section Layer6_s2tte_pa_LowSpec.
   Context `{int_ptr: IntPtrCast}.
 
   Definition s2tte_pa_spec_low (v_0: Z) (v_1: Z) (st: RData) : (option (Z * RData)) :=
-    if ((v_1 <? (3)) && (((v_0 & (3)) =? (3))))
-    then (Some (((v_0 & (281474976710655)) & (((- 1) << (12)))), st))
-    else (Some (((v_0 & (281474976710655)) & (((- 1) << (((((3 - (v_1)) * (9)) + (12)) & (4294967295)))))), st)).
+    when v_4, st_0 == ((s2tte_is_table_spec v_0 v_1 st));
+    if v_4
+    then (
+      when v_6, st_1 == ((addr_level_mask_spec v_0 3 st_0));
+      (Some (v_6, st_1)))
+    else (
+      when v_8, st_1 == ((addr_level_mask_spec v_0 v_1 st_0));
+      (Some (v_8, st_1))).
 
 End Layer6_s2tte_pa_LowSpec.
 
