container/coq/pointer/Layer7/Spec.v
@@ -27,7 +27,7 @@ Section Layer7_Spec.
       else (Some (false, st))).
 
   Definition s2tte_create_table_spec_abs (v_0: abs_PA_t) (v_1: Z) (st: RData) : (option (abs_PTE_t * RData)) :=
-    (Some ((mkabs_PTE_t v_0 3 0), st)).
+    (Some ((mkabs_PTE_t v_0 3 0 0), st)).
 
   Definition rtt_create_internal_spec_abs (v_0: Ptr) (v_1_abs: abs_PA_t) (v_2: Z) (v_3: Z) (v_4: Z) (st: RData) : (option (Z * RData)) :=
     when ret, st' == ((granule_try_lock_spec (mkPtr "granules" (v_1_abs.(meta_granule_offset))) 1 st));
@@ -71,7 +71,7 @@ Section Layer7_Spec.
                     ((((st_10.(share)).(granule_data)) @ ((((ret_record.(e_2)).(poffset)) + ((8 * ((ret_record.(e_3)))))) / (4096))).[g_norm] :<
                       (((((st_10.(share)).(granule_data)) @ ((((ret_record.(e_2)).(poffset)) + ((8 * ((ret_record.(e_3)))))) / (4096))).(g_norm)) #
                         ((((ret_record.(e_2)).(poffset)) + ((8 * ((ret_record.(e_3)))))) mod (4096)) ==
-                        (test_PTE_Z (mkabs_PTE_t v_1_abs 3 0))))))));
+                        (test_PTE_Z (mkabs_PTE_t v_1_abs 3 0 0))))))));
           when st_17 == ((granule_unlock_spec (mkPtr "granules" (v_1_abs.(meta_granule_offset))) st_16));
           (Some (0, st_17)))
         else (
@@ -104,7 +104,7 @@ Section Layer7_Spec.
                           ((((st_10.(share)).(granule_data)) @ ((((ret_record.(e_2)).(poffset)) + ((8 * ((ret_record.(e_3)))))) / (4096))).[g_norm] :<
                             (((((st_10.(share)).(granule_data)) @ ((((ret_record.(e_2)).(poffset)) + ((8 * ((ret_record.(e_3)))))) / (4096))).(g_norm)) #
                               ((((ret_record.(e_2)).(poffset)) + ((8 * ((ret_record.(e_3)))))) mod (4096)) ==
-                              (test_PTE_Z (mkabs_PTE_t v_1_abs 3 0))))))));
+                              (test_PTE_Z (mkabs_PTE_t v_1_abs 3 0 0))))))));
                 when st_15 == ((granule_unlock_spec (mkPtr "granules" (v_1_abs.(meta_granule_offset))) st_14));
                 (Some (0, st_15)))
             | None => None
@@ -123,7 +123,7 @@ Section Layer7_Spec.
                       ((((st_4.(share)).(granule_data)) @ ((((ret_record.(e_2)).(poffset)) + ((8 * ((ret_record.(e_3)))))) / (4096))).[g_norm] :<
                         (((((st_4.(share)).(granule_data)) @ ((((ret_record.(e_2)).(poffset)) + ((8 * ((ret_record.(e_3)))))) / (4096))).(g_norm)) #
                           ((((ret_record.(e_2)).(poffset)) + ((8 * ((ret_record.(e_3)))))) mod (4096)) ==
-                          (test_PTE_Z (mkabs_PTE_t v_1_abs 3 0))))))));
+                          (test_PTE_Z (mkabs_PTE_t v_1_abs 3 0 0))))))));
             when st_15 == ((granule_unlock_spec (mkPtr "granules" (v_1_abs.(meta_granule_offset))) st_14));
             (Some (0, st_15)))))
       else (
@@ -192,7 +192,7 @@ Section Layer7_Spec.
                             ((((st_11.(share)).(granule_data)) @ ((((ret_record.(e_2)).(poffset)) + ((8 * ((ret_record.(e_3)))))) / (4096))).[g_norm] :<
                               (((((st_11.(share)).(granule_data)) @ ((((ret_record.(e_2)).(poffset)) + ((8 * ((ret_record.(e_3)))))) / (4096))).(g_norm)) #
                                 ((((ret_record.(e_2)).(poffset)) + ((8 * ((ret_record.(e_3)))))) mod (4096)) ==
-                                (test_PTE_Z (mkabs_PTE_t v_1_abs 3 0))))))));
+                                (test_PTE_Z (mkabs_PTE_t v_1_abs 3 0 0))))))));
                   when st_18 == ((granule_unlock_spec (mkPtr "granules" (v_1_abs.(meta_granule_offset))) st_17));
                   (Some (0, st_18)))
                 else (
@@ -225,7 +225,7 @@ Section Layer7_Spec.
                                   ((((st_11.(share)).(granule_data)) @ ((((ret_record.(e_2)).(poffset)) + ((8 * ((ret_record.(e_3)))))) / (4096))).[g_norm] :<
                                     (((((st_11.(share)).(granule_data)) @ ((((ret_record.(e_2)).(poffset)) + ((8 * ((ret_record.(e_3)))))) / (4096))).(g_norm)) #
                                       ((((ret_record.(e_2)).(poffset)) + ((8 * ((ret_record.(e_3)))))) mod (4096)) ==
-                                      (test_PTE_Z (mkabs_PTE_t v_1_abs 3 0))))))));
+                                      (test_PTE_Z (mkabs_PTE_t v_1_abs 3 0 0))))))));
                         when st_16 == ((granule_unlock_spec (mkPtr "granules" (v_1_abs.(meta_granule_offset))) st_15));
                         (Some (0, st_16)))
                     | None => None
@@ -244,7 +244,7 @@ Section Layer7_Spec.
                               ((((st_5.(share)).(granule_data)) @ ((((ret_record.(e_2)).(poffset)) + ((8 * ((ret_record.(e_3)))))) / (4096))).[g_norm] :<
                                 (((((st_5.(share)).(granule_data)) @ ((((ret_record.(e_2)).(poffset)) + ((8 * ((ret_record.(e_3)))))) / (4096))).(g_norm)) #
                                   ((((ret_record.(e_2)).(poffset)) + ((8 * ((ret_record.(e_3)))))) mod (4096)) ==
-                                  (test_PTE_Z (mkabs_PTE_t v_1_abs 3 0))))))));
+                                  (test_PTE_Z (mkabs_PTE_t v_1_abs 3 0 0))))))));
                     when st_16 == ((granule_unlock_spec (mkPtr "granules" (v_1_abs.(meta_granule_offset))) st_15));
                     (Some (0, st_16)))))
             | None => None
@@ -254,6 +254,12 @@ Section Layer7_Spec.
             when st_8 == ((granule_unlock_spec (mkPtr "granules" (v_1_abs.(meta_granule_offset))) st_7));
             (Some ((pack_struct_return_code_para (make_return_code_para 8)), st_8))))))
     else (Some ((pack_struct_return_code_para (make_return_code_para 1)), st')).
+
+  Definition set_pas_any_to_ns_spec (v_0: Z) (st: RData) : (option RData) :=
+    (Some st).
+
+  Definition set_pas_ns_to_any_spec (v_0: Z) (st: RData) : (option RData) :=
+    (Some st).
 
   Definition smc_granule_ns_to_any_spec_abs (v_0: Z) (v_1_abs: abs_PA_t) (st: RData) : (option (Z * RData)) :=
     when st_1 == ((spinlock_acquire_spec (mkPtr "granules" (v_1_abs.(meta_granule_offset))) st));
@@ -342,19 +348,17 @@ Section Layer7_Spec.
       then (Some (true, st))
       else (Some (false, st))).
 
-  Definition smc_granule_ns_to_any_spec (v_0: Z) (st: RData) : (option (Z * RData)) :=
-    None.
-
-  Definition smc_granule_any_to_ns_spec (v_0: Z) (st: RData) : (option (Z * RData)) :=
-    None.
+  Definition s2tte_is_assigned_spec (v_0: Z) (v_1: Z) (st: RData) : (option (bool * RData)) :=
+    (Some (((v_0 & (63)) =? (4)), st)).
 
 End Layer7_Spec.
 
 #[global] Hint Unfold s1tte_is_valid_spec_abs: spec.
 #[global] Hint Unfold s2tte_create_table_spec_abs: spec.
 #[global] Hint Unfold rtt_create_internal_spec_abs: spec.
+#[global] Hint Unfold set_pas_any_to_ns_spec: spec.
+#[global] Hint Unfold set_pas_ns_to_any_spec: spec.
 #[global] Hint Unfold smc_granule_ns_to_any_spec_abs: spec.
 #[global] Hint Unfold smc_granule_any_to_ns_spec_abs: spec.
 #[global] Hint Unfold s1tte_is_valid_spec: spec.
-#[global] Hint Unfold smc_granule_ns_to_any_spec: spec.
-#[global] Hint Unfold smc_granule_any_to_ns_spec: spec.
+#[global] Hint Unfold s2tte_is_assigned_spec: spec.
