container/coq/pointer/Layer8/update_ripas/LowSpec.v
@@ -1,0 +1,19 @@
+Require Import Code.
+Require Import CommonDeps.
+Require Import DataTypes.
+Require Import GlobalDefs.
+
+Local Open Scope string_scope.
+Local Open Scope Z_scope.
+
+Section Layer8_update_ripas_LowSpec.
+
+  Context `{int_ptr: IntPtrCast}.
+
+  Definition update_ripas_spec_low (v_0: Ptr) (v_1: Z) (v_2: Z) (st: RData) : (option (bool * RData)) :=
+    when ret, pte == ((update_ripas_spec_abs (test_Ptr_PTE v_0) v_1 v_2 st));
+    (Some (ret, st)).
+
+End Layer8_update_ripas_LowSpec.
+
+#[global] Hint Unfold update_ripas_spec_low: spec.
