container/coq/pointer/Layer9/rsi_rtt_set_ripas/CodeProof.v
@@ -1,0 +1,26 @@
+Require Import Code.
+Require Import CommonDeps.
+Require Import DataTypes.
+Require Import GlobalDefs.
+Require Import Layer8.Layer.
+Require Import Layer9.rsi_rtt_set_ripas.LowSpec.
+Require Import Zwf.
+
+Local Open Scope string_scope.
+Local Open Scope Z_scope.
+Local Opaque Z.add Z.mul Z.div Z.sub Z.land Z.lor Z.lxor Z.shiftl Z.shiftr Z.quot Z.rem Z.testbit Z.setbit Z.clearbit xorb List.nth.
+
+Section Layer9_rsi_rtt_set_ripas_CodeProof.
+
+  Context `{int_ptr: IntPtrCast}.
+
+    Lemma f_rsi_rtt_set_ripas_correct:
+      forall v_0 v_1 v_2 v_3 st st' res
+             (Hspec: rsi_rtt_set_ripas_spec_low v_0 v_1 v_2 v_3 st = Some (res, st')),
+        exec_func Layer8_layer code "rsi_rtt_set_ripas"
+                  [VInt v_0; VInt v_1; VInt v_2; VInt v_3]
+                  st st' (Some (VInt res)).
+Admitted.
+
+End Layer9_rsi_rtt_set_ripas_CodeProof.
+
